@prefix ceterms: <http://purl.org/ctdl/terms/> .
@prefix dct: <http://purl.org/dc/terms/> .
@prefix jdx: <http://purl.org/jdx/terms/> .
@prefix owl: <http://www.w3.org/2002/07/owl#> .
@prefix rdf: <http://www.w3.org/1999/02/22-rdf-syntax-ns#> .
@prefix rdfs: <http://www.w3.org/2000/01/rdf-schema#> .
@prefix schema: <http://schema.org/> .
@prefix skos: <http://www.w3.org/2004/02/skos/core#> .
@prefix xsd: <http://www.w3.org/2001/XMLSchema#> .

jdx:AnnotatedDefinedTerm a rdfs:Class ;
    rdfs:label "Annotated Defined Term"@en-US ;
    dct:identifier "jdx:AnnotatedDefinedTerm" ;
    rdfs:comment "Word, name, acronym, phrase, defined in a controlled value space (e.g., taxonomy, glossary, dictionary, tag list, and other forms of enumeration)."@en-US ;
    rdfs:isDefinedBy jdx: ;
    skos:scopeNote "Used in the context of JDX to assign terms from occupation, industry and instructional program classifications, skills and abilities, and abstract concepts to JDX entities. Through the class' relationship with the jdx:ScaledAnnotation class, terms can be conditioned through applications of scales for attributes such as importance and frequency."@en-US .

jdx:AssessmentProfile a rdfs:Class ;
    rdfs:label "Assessment Profile"@en-US ;
    dct:identifier "jdx:AssessmentProfile" ;
    rdfs:comment "Entity that describes the key characteristics of an assessment administered to candidates for a job."@en-US ;
    rdfs:isDefinedBy jdx: .

jdx:Condition a rdfs:Class ;
    rdfs:label "Condition"@en-US ;
    dct:identifier "jdx:Condition"@en-US ;
    rdfs:comment "Entity providing the means to make logical asserions that combine resources that in aggregate fulfill education, experience and credential requirements."@en-US ;
    rdfs:isDefinedBy jdx: .

jdx:Credential a rdfs:Class ;
    rdfs:label "Credential"@en-US ;
    dct:identifier "jdx:Credential" ;
    rdfs:comment "Entity describing authoritative permission to hold a certain status or to do certain things, e.g. to practice some trade or profession."@en-US ;
    rdfs:isDefinedBy jdx: .

jdx:Job a rdfs:Class ;
    rdfs:label "Job"@en-US ;
    dct:identifier "jdx:Job" ;
    rdfs:comment "Formally defined and titled role for performing a set of work tasks or activities."@en-US ;
    rdfs:isDefinedBy jdx: ;
    skos:scopeNote "The jdx:JobDescription, jdx:JobCompetencyProfile and jdx:JobPosting define windows into the content of the jdx:Job; do NOT use jdx:Job as an entity in any public facing resource. Entity used internally as \"master\" to which all properties used in JobDescription, JobPosting, and JobCompetencyProfile are applicable."@en-US .

jdx:JobCompetencyProfile a rdfs:Class ;
    rdfs:label "Job Competency Profile"@en-US ;
    dct:identifier "jdx:JobCompetencyProfile" ;
    rdfs:comment "Entity listing major work tasks, knowledge, skills, and abilities requirements for carrying out those work tasks based on a job analysis that engages subject matter experts in defining and validating the importance, frequency, or other types of weightings of the enumerated competencies."@en-US ;
    rdfs:isDefinedBy jdx: .

jdx:JobDescription a rdfs:Class ;
    rdfs:label "Job Description"@en-US ;
    dct:identifier "jdx:JobDescription" ;
    rdfs:comment "Entity providing a statement of a job position generally including the formal job title, duties, purpose, responsibilities, scope, reporting relationships and working conditions along with the knowledge, skills, abilities, education, qualifications, experience and other requirements for performing the job."@en-US ;
    rdfs:isDefinedBy jdx: .

jdx:JobPosting a rdfs:Class ;
    rdfs:label "Job Posting"@en-US ;
    dct:description "Entity that contains information on the employer and the job position based on a job description as well as how to apply for the job opening and how long the posting is valid."@en-US ;
    dct:identifier "jdx:JobPosting" ;
    rdfs:comment "Entity describing an on-line advertisement for filling one or more job openings."@en-US ;
    rdfs:isDefinedBy jdx: .

jdx:PostingInstructions a rdfs:Class ;
    rdfs:label "Posting Instructions"@en-US ;
    dct:identifier "jdx:PostingInstructions" ;
    rdfs:comment "Entity providing information about where and how a posting should be communicated."@en-US ;
    rdfs:isDefinedBy jdx: ;
    skos:scopeNote "A posting channel usually would be a job board or other advertising medium (HR)."@en-US .

jdx:QualifyingExperience a rdfs:Class ;
    rdfs:label "QualifyingExperience"@en-US ;
    dct:identifier "jdx:QualifyingExperience" ;
    rdfs:comment "Entity describing verifiable work, education or training experience supporting a person's qualification to perform the tasks and responsibilities of a position."@en-US ;
    rdfs:isDefinedBy jdx: ;
    skos:scopeNote "A QualifyingExperience that results in the award of some form of credential should use the jdx:Credential class to describe that award."@en-US .

jdx:ScaleAnnotation a rdfs:Class ;
    rdfs:label "Scale Annotation"@en-US ;
    dct:identifier "jdx:ScaleAnnotation" ;
    rdfs:comment "Resource for identifying and applying a defined scale or rating to another resource."@en-US ;
    rdfs:isDefinedBy jdx: ;
    skos:scopeNote "Used, for example, when applying an importance scale to a competency identified in an instance of the AnnotatedDefinedTerm class."@en-US .

schema:ContactPoint a rdfs:Class ;
    rdfs:label "Contact Point"@en-US ;
    dct:identifier "schema:ContactPoint" ;
    rdfs:comment "Contact point—for example, for information about a job opening or interview."@en-US ;
    rdfs:isDefinedBy schema: .

schema:DefinedTermSet a rdfs:Class ;
    rdfs:label "Defined Term Set"@en-US ;
    dct:identifier "schema:DefinedTermSet" ;
    rdfs:comment "A set of defined terms for example a set of categories or a classification scheme, a glossary, dictionary or enumeration."@en-US ;
    rdfs:isDefinedBy schema: .

schema:GeoCoordinates a rdfs:Class ;
    rdfs:label "Location Geocoordinates"@en-US ;
    dct:identifier "schema:GeoCoordinates" ;
    rdfs:comment "Geographic coordinates of a place or event."@en-US ;
    rdfs:isDefinedBy schema: ;
    skos:scopeNote "Use to identify a place using geo coordinates; preferably includes a URI for the location as well as longitude and latitude from a service such as GeoNames (https://www.geonames.org/)."@en-US .

schema:MonetaryAmount a rdfs:Class ;
    rdfs:label "Monetary Amount"@en-US ;
    dct:identifier "schema:MonetaryAmount" ;
    rdfs:comment "A monetary value or range."@en-US ;
    rdfs:isDefinedBy schema: ;
    skos:scopeNote "This type can be used to describe an amount of money such as $50 USD, or a range as in describing a bank account being suitable for a balance between £1,000 and £1,000,000 GBP, or the value of a salary, etc."@en-US .

schema:MonetaryAmountDistribution a rdfs:Class ;
    rdfs:label "Monetary Amount Distribution"@en-US ;
    dct:identifier "schema:MonetaryAmountDistribution" ;
    rdfs:comment "Statistical distribution of monetary amounts."@en-US ;
    rdfs:isDefinedBy schema: .

schema:Organization a rdfs:Class ;
    rdfs:label "Organization"@en-US ;
    dct:identifier "schema:Organization"@en-US ;
    rdfs:comment "An organization such as a corporate body, employer, distribution channel provider."@en-US ;
    rdfs:isDefinedBy schema: .

schema:Place a rdfs:Class ;
    rdfs:label "Location"@en-US ;
    dct:identifier "schema:Place" ;
    rdfs:comment "Fixed physical location."@en-US ;
    rdfs:isDefinedBy schema: .

schema:PostalAddress a rdfs:Class ;
    rdfs:label "Postal Address"@en-US ;
    dct:identifier "schema:PostalAddress" ;
    rdfs:comment "Mailing address of an entity."@en-US ;
    rdfs:isDefinedBy schema: .

schema:PropertyValue a rdfs:Class ;
    rdfs:label "Property Value"@en-US ;
    dct:description "Entity provides the means to define a needed property not otherwise defined in the JDX schema or profile."@en-US ;
    dct:identifier "schema:PropertyValue" ;
    rdfs:comment "Property-value pair, e.g. representing a feature of an entity."@en-US ;
    rdfs:isDefinedBy schema: ;
    skos:scopeNote "Use PropertyValue sparingly! Always use a specific property from a known namespace when they serve your purpose. Using PropertyValue as a substitute for such properties will not trigger the same linked data function as the predicate of an RDF triple as will a more specific property."@en-US .

schema:QuantitativeValue a rdfs:Class ;
    rdfs:label "Quantitative Value"@en-US ;
    dct:identifier "schema:QuantitativeValue" ;
    rdfs:comment "Point value or interval for product characteristics and other purposes."@en-US ;
    rdfs:isDefinedBy schema: .

jdx:ability a rdfs:Property ;
    rdfs:label "Ability"@en-US ;
    dct:identifier "jdx:ability" ;
    rdfs:comment "Aptitude, capacity or power to act physically, socially, mentally, legally, or morally at a level suitable to the work context; select from an existing enumeration of such types."@en-US ;
    rdfs:domain jdx:Job ;
    rdfs:isDefinedBy jdx: ;
    rdfs:range jdx:AnnotatedDefinedTerm ;
    rdfs:subPropertyOf jdx:competency ;
    skos:scopeNote "Use a value selected from a controlled vocabulary of ability types such as the O*NET cognitive, sensory, psychomotor and physical abilities; encode using the jdx:AnnotatedDefinedTerm entity."@en-US .

jdx:acquiredInternally a rdfs:Property ;
    rdfs:label "Acquired Internally"@en-US ;
    dct:identifier "jdx:acquiredInternally" ;
    rdfs:comment "Whether or not a requirement in a posting may be acquired post-hire."@en-US ;
    rdfs:domain jdx:ScaleAnnotation ;
    rdfs:isDefinedBy jdx: ;
    rdfs:range xsd:boolean .

jdx:acquisitionDifficulty a rdfs:Property ;
    rdfs:label "Acquisition Difficulty"@en-US ;
    dct:identifier "jdx:acquisitionDifficulty" ;
    rdfs:comment "Rating or score representing the difficulty of the particular entity to acquire."@en-US ;
    rdfs:domain jdx:ScaleAnnotation ;
    rdfs:isDefinedBy jdx: ;
    rdfs:range xsd:float ;
    skos:scopeNote "The scale may be applied to any appropriate controlled vocabulary concept such as knowledge, skill, and ability as identified in the associated jdx:AnnotationDefinedTerm."@en-US .

jdx:alternativeCondition a rdfs:Property ;
    rdfs:label "Alternative Condition"@en-US ;
    dct:identifier "jdx:alternativeCondition" ;
    rdfs:comment "Resource referenced provides the means to make logical asserions about alternative conditions."@en-US ;
    rdfs:domain jdx:Condition ;
    rdfs:isDefinedBy jdx: ;
    rdfs:range jdx:Condition .

jdx:alternativeCredential a rdfs:Property ;
    rdfs:label "Alternative Credential"@en-US ;
    dct:identifier "jdx:alternativeCredential" ;
    rdfs:comment "Description of an alternative credential fulfilling requirements for the position or occupation."@en-US ;
    rdfs:domain jdx:Condition,
        jdx:Job,
        jdx:JobDescription,
        jdx:JobPosting ;
    rdfs:isDefinedBy jdx: ;
    rdfs:range jdx:Credential .

jdx:alternativeEducation a rdfs:Property ;
    rdfs:label "Alternative Education"@en-US ;
    dct:identifier "jdx:alternativeEducation" ;
    rdfs:comment "Description of an alternative education or training fulfilling requirements for the position or occupation."@en-US ;
    rdfs:domain jdx:Condition,
        jdx:Job,
        jdx:JobDescription,
        jdx:JobPosting ;
    rdfs:isDefinedBy jdx: ;
    rdfs:range jdx:QualifyingExperience .

jdx:alternativeExperience a rdfs:Property ;
    rdfs:label "Alternative Experience"@en-US ;
    dct:identifier "jdx:alternativeExperience" ;
    rdfs:comment "Description of an alternative experience fulfilling requirements for the position or occupation."@en-US ;
    rdfs:domain jdx:Condition,
        jdx:Job,
        jdx:JobDescription,
        jdx:JobPosting ;
    rdfs:isDefinedBy jdx: ;
    rdfs:range jdx:QualifyingExperience .

jdx:annotation a rdfs:Property ;
    rdfs:label "Related Annotation"@en-US ;
    dct:identifier "jdx:annotation" ;
    rdfs:comment "Entity providing qualifying notations including application of scales and other weights to concepts and competencies identified through a jdx:AnnotatedDefinedTerm."@en-US ;
    rdfs:domain jdx:AnnotatedDefinedTerm ;
    rdfs:isDefinedBy jdx: ;
    rdfs:range jdx:ScaleAnnotation .

jdx:applicantLocationRequirement a rdfs:Property ;
    rdfs:label "Applicant Location Requirement"@en-US ;
    dct:identifier "jdx:applicantLocationRequirement" ;
    rdfs:comment "Geographic location(s) in which employees may be located for remote (telecommuting) jobs."@en-US ;
    rdfs:domain jdx:Job,
        jdx:JobPosting ;
    rdfs:isDefinedBy jdx: ;
    rdfs:range schema:GeoCoordinates .

jdx:applicationCloseDate a rdfs:Property ;
    rdfs:label "Application Close Data"@en-US ;
    dct:identifier "jdx:applicationCloseDate" ;
    rdfs:comment "Closing date for accepting applications."@en-US ;
    rdfs:domain jdx:PostingInstructions ;
    rdfs:isDefinedBy jdx: ;
    rdfs:range xsd:dateTime .

jdx:applicationContact a rdfs:Property ;
    rdfs:label "Contact Point"@en-US ;
    dct:identifier "jdx:applicationContact" ;
    rdfs:comment "Organization or person contact point for the posting."@en-US ;
    rdfs:domain jdx:PostingInstructions ;
    rdfs:isDefinedBy jdx: ;
    rdfs:range schema:ContactPoint .

jdx:applicationInstructions a rdfs:Property ;
    rdfs:label "Application Instructions"@en-US ;
    dct:identifier "jdx:applicationInstructions" ;
    rdfs:comment "Narrative instructions for applying for this position."@en-US ;
    rdfs:domain jdx:PostingInstructions ;
    rdfs:isDefinedBy jdx: ;
    rdfs:range rdf:langString .

jdx:applicationLocation a rdfs:Property ;
    rdfs:label "Application Location"@en-US ;
    dct:identifier "jdx:applicationLocation" ;
    rdfs:comment "Physical location where job applications can be submitted."@en-US ;
    rdfs:domain jdx:PostingInstructions ;
    rdfs:isDefinedBy jdx: ;
    rdfs:range schema:Place .

jdx:areaAssessed a rdfs:Property ;
    rdfs:label "Area Assessed"@en-US ;
    dct:identifier "jdx:areaAssessed" ;
    rdfs:comment "Description of the area or domain to be assessed."@en-US ;
    rdfs:domain jdx:AssessmentProfile ;
    rdfs:isDefinedBy jdx: ;
    rdfs:range rdf:langString .

jdx:assessmentExample a rdfs:Property ;
    rdfs:label "Assessment Example"@en-US ;
    dct:identifier "jdx:assessmentExample" ;
    rdfs:comment "Resource describing an example assessment."@en-US ;
    rdfs:domain jdx:AssessmentProfile ;
    rdfs:isDefinedBy jdx: ;
    rdfs:range xsd:anyURI .

jdx:assessmentMethod a rdfs:Property ;
    rdfs:label "Assessment Method"@en-US ;
    dct:identifier "jdx:assessmentMethod" ;
    rdfs:comment "Type of method used to conduct an assessment; select from an existing enumeration of such types."@en-US ;
    rdfs:domain jdx:AssessmentProfile,
        jdx:ScaleAnnotation ;
    rdfs:isDefinedBy jdx: ;
    rdfs:range jdx:AnnotatedDefinedTerm ;
    skos:scopeNote "Use a value selected from a controlled vocabulary of assessment method types such as the ceterms:AssessmentMethod vocabulary; encode using the jdx:AnnotatedDefinedTerm entity."@en-US .

jdx:attitude a rdfs:Property ;
    rdfs:label "Attitude"@en-US ;
    dct:identifier "jdx:attitude" ;
    rdfs:comment "Motivator of performance including values, aspirations, and priorities necessary to successful performance of a task or job; select from an existing enumeration of such types."@en-US ;
    rdfs:domain jdx:Job ;
    rdfs:isDefinedBy jdx: ;
    rdfs:range jdx:AnnotatedDefinedTerm ;
    rdfs:subPropertyOf jdx:competency ;
    skos:scopeNote "Use a value selected from a controlled vocabulary of attitude types; encode using the jdx:AnnotatedDefinedTerm entity."@en-US .

jdx:careerLevel a rdfs:Property ;
    rdfs:label "Career Level"@en-US ;
    dct:identifier "jdx:careerLevel" ;
    rdfs:comment "A code classifying the level of a candidate based on career experience; select from an existing enumeration of such types."@en-US ;
    rdfs:domain jdx:Job ;
    rdfs:isDefinedBy jdx: ;
    rdfs:range jdx:AnnotatedDefinedTerm ;
    skos:scopeNote "Use a value selected from a controlled vocabulary of career level types (e.g., HR Open Standards CareerLevelCodeList.json); encode using the jdx:AnnotatedDefinedTerm entity."@en-US .

jdx:citizenshipRequirement a rdfs:Property ;
    rdfs:label "Citizenship Requirement"@en-US ;
    dct:identifier "jdx:citizenshipRequirement" ;
    rdfs:comment "Required country of the applicant's citizenship."@en-US ;
    rdfs:domain jdx:Job,
        jdx:JobDescription,
        jdx:JobPosting ;
    rdfs:isDefinedBy jdx: ;
    rdfs:range jdx:AnnotatedDefinedTerm ;
    skos:scopeNote "Use a value selected from a country code list such as the Library of Congress' List of Countries (http://id.loc.gov/vocabulary/countries.html)."@en-US .

jdx:conceptKeyword a rdfs:Property ;
    rdfs:label "Concept Keyword"@en-US ;
    dct:identifier "jdx:conceptKeyword" ;
    rdfs:comment "Word or phrase used to refine and describe significant aspects of the entity."@en-US ;
    rdfs:domain jdx:AssessmentProfile ;
    rdfs:isDefinedBy jdx: ;
    rdfs:range rdf:langString .

jdx:credentialCategory a rdfs:Property ;
    rdfs:label "Credential Category"@en-US ;
    dct:identifier "jdx:credentialCategory" ;
    rdfs:comment "Type of credential such as badge, certification, bachelor degree; select from an existing enumeration of such types."@en-US ;
    rdfs:domain jdx:Credential ;
    rdfs:isDefinedBy jdx: ;
    rdfs:range jdx:AnnotatedDefinedTerm ;
    owl:equivalentProperty: "http://purl.org/ctdl/terms/credentialType" ;
    skos:scopeNote "Use a value selected from a controlled vocabulary of credential types (e.g., credential subclasses from CTDL); encode using the jdx:AnnotatedDefinedTerm entity."@en-US .

jdx:derivedFrom a rdfs:Property ;
    rdfs:label "Derived From"@en-US ;
    dct:identifier "jdx:derivedFrom" ;
    rdfs:comment "Identifies a resource from which properties of the resource being described were obtained in whole or in part."@en-US ;
    rdfs:domain jdx:JobCompetencyProfile,
        jdx:JobDescription,
        jdx:JobPosting ;
    rdfs:isDefinedBy jdx: ;
    rdfs:range jdx:Job .

jdx:disclaimer a rdfs:Property ;
    rdfs:label "Description"@en-US ;
    dct:identifier "jdx:disclaimer" ;
    rdfs:comment "Statement that denies aspects of a statement made or omitted by the employing entity in the position or posting."@en-US ;
    rdfs:domain jdx:Job,
        jdx:JobDescription,
        jdx:JobPosting ;
    rdfs:isDefinedBy jdx: ;
    rdfs:range rdf:langString .

jdx:distributionChannel a rdfs:Property ;
    rdfs:label "Distribution Channel"@en-US ;
    dct:identifier "jdx:distributionChannel" ;
    rdfs:comment "Identifies a job board or media channel associated with a job posting."@en-US ;
    rdfs:domain jdx:PostingInstructions ;
    rdfs:isDefinedBy jdx: ;
    rdfs:range xsd:anyURI .

jdx:educationLevel a rdfs:Property ;
    rdfs:label "Education Level"@en-US ;
    dct:identifier "schema:educationLevel" ;
    rdfs:comment "Word or phrase identifying the location of the person in terms of his or her progression through an education or training context; select from an existing enumeration of such types."@en-US ;
    rdfs:domain jdx:Job,
        jdx:JobDescription,
        jdx:JobPosting,
        jdx:QualifyingExperience ;
    rdfs:isDefinedBy jdx: ;
    rdfs:range jdx:AnnotatedDefinedTerm ;
    skos:scopeNote "Use a value selected from a controlled vocabulary of education levels such as ceterms:AudienceLevel or HR Open Standards IscedCodeList.json; encode using the jdx:AnnotatedDefinedTerm entity."@en-US .

jdx:employerOverview a rdfs:Property ;
    rdfs:label "Employer Overview"@en-US ;
    dct:identifier "jdx:employerOverview" ;
    rdfs:comment "Description of the employer, career opportunities and work environment."@en-US ;
    rdfs:domain jdx:Job,
        jdx:JobPosting ;
    rdfs:isDefinedBy <https://schema.org/> ;
    rdfs:range rdf:langString .

jdx:employmentUnit a rdfs:Property ;
    rdfs:label "Employment Unit"@en-US ;
    dct:identifier "jdx:employmentUnit" ;
    rdfs:comment "Department, unit and/or facility where the employee reports and/or in which the job is to be performed."@en-US ;
    rdfs:domain jdx:Job,
        jdx:JobDescription,
        jdx:JobPosting ;
    rdfs:isDefinedBy jdx: ;
    rdfs:range schema:Organization .

jdx:equivalentCredential a rdfs:Property ;
    rdfs:label "Equivalent Credential"@en-US ;
    dct:identifier "jdx:equivalentCredential" ;
    rdfs:comment "Description of an equivalent credential for the position or occupation."@en-US ;
    rdfs:domain jdx:Condition,
        jdx:Job,
        jdx:JobDescription,
        jdx:JobPosting ;
    rdfs:isDefinedBy jdx: ;
    rdfs:range jdx:Credential .

jdx:equivalentEducation a rdfs:Property ;
    rdfs:label "Equivalent Education"@en-US ;
    dct:identifier "jdx:equivalentEducation" ;
    rdfs:comment "Description of equivalent education or training for the position or occupation."@en-US ;
    rdfs:domain jdx:Condition,
        jdx:Job,
        jdx:JobDescription,
        jdx:JobPosting ;
    rdfs:isDefinedBy jdx: ;
    rdfs:range jdx:QualifyingExperience ;
    skos:scopeNote "An educational experience <u>without</u> award of a credential should be recorded with a range of jdx:QualifyingExperience. An educational experience <u>with</u> award of a credential should be recoded with a range of jdxCredential, not jdx:QualifyingExperience."@en-US .

jdx:equivalentExperience a rdfs:Property ;
    rdfs:label "Equivalent Experience"@en-US ;
    dct:identifier "jdx:equivalentEperience" ;
    rdfs:comment "Description of equivalent experience for the position or occupation."@en-US ;
    rdfs:domain jdx:Condition,
        jdx:Job,
        jdx:JobDescription,
        jdx:JobPosting ;
    rdfs:isDefinedBy jdx: ;
    rdfs:range jdx:QualifyingExperience .

jdx:evidence a rdfs:Property ;
    rdfs:label "Evidence"@en-US ;
    dct:identifier "jdx:evidence" ;
    rdfs:comment "Referenced artifact or performance confirming or supporting an assertion."@en-US ;
    rdfs:domain jdx:Credential,
        jdx:QualifyingExperience ;
    rdfs:isDefinedBy jdx: ;
    rdfs:range xsd:anyURI .

jdx:evidenceCategory a rdfs:Property ;
    rdfs:label "EvidenceType"@en-US ;
    dct:identifier "jdx:evidenceType" ;
    rdfs:comment "The type of referenced artifact, exam or performance confirming or supporting an assertion; select from an existing enumeration of such types."@en-US ;
    rdfs:domain jdx:AssessmentProfile,
        jdx:Credential,
        jdx:QualifyingExperience,
        jdx:ScaleAnnotation ;
    rdfs:isDefinedBy jdx: ;
    rdfs:range jdx:AnnotatedDefinedTerm ;
    skos:scopeNote "Use a value selected from a controlled vocabulary of evidence types; encode using the jdx:AnnotatedDefinedTerm entity."@en-US .

jdx:experienceCategory a rdfs:Property ;
    rdfs:label "Experience Category"@en-US ;
    dct:identifier "jdx:experienceCategory" ;
    rdfs:comment "Category of experience needed for the position or Occupation; select from an existing enumeration of such types."@en-US ;
    rdfs:domain jdx:Job,
        jdx:JobDescription,
        jdx:JobPosting,
        jdx:QualifyingExperience ;
    rdfs:isDefinedBy jdx: ;
    rdfs:range jdx:AnnotatedDefinedTerm ;
    skos:scopeNote "Use a value selected from a controlled vocabulary of experience types including, but not limited to, \"Education Experience\", \"Training Experience\", \"Work Experience\" and it's subtypes \"Apprenticeship\" and \"Traineeship\"; encode using the jdx:AnnotatedDefinedTerm entity."@en-US .

jdx:fein a rdfs:Property ;
    rdfs:label "FEIN"@en-US ;
    dct:identifier "jdx:fein" ;
    rdfs:comment "Federal Employer Identification Number (FEIN) identifying organizations, persons, states, government agencies, corporations, and companies."@en-US ;
    rdfs:domain schema:Organization ;
    rdfs:isDefinedBy jdx: ;
    rdfs:range xsd:string ;
    owl:equivalentProperty: "http://purl.org/ctdl/terms/fein" .

jdx:formattedDescription a rdfs:Property ;
    rdfs:label "Formatted Description"@en-US ;
    dct:identifier "jdx:formattedDescription" ;
    rdfs:comment "HTML-tagged summary of the salient aspects of the job, including job responsibilities, qualifications, skills, working hours, education requirements, and experience requirements."@en-US ;
    rdfs:domain jdx:Job,
        jdx:JobPosting ;
    rdfs:isDefinedBy jdx: ;
    rdfs:range rdf:HTML ;
    skos:scopeNote "For language-tagged descriptions without embedded HTML markup, use the schema:description property."@en-US .

jdx:hasCompetencyProfile a rdfs:Property ;
    rdfs:label "Has Competency Profile"@en-US ;
    dct:identifier "jdx:hasCompetencyProfile" ;
    rdfs:comment "Referenced resource describes the major work tasks, knowledge, skills, and abilities requirements for carrying out those work tasks based on a job analysis that engages subject matter experts in defining and validating the importance, frequency, or other types of weightings of the enumerated competencies."@en-US ;
    rdfs:domain jdx:Job,
        jdx:JobDescription ;
    rdfs:isDefinedBy jdx: ;
    rdfs:range jdx:JobCompetencyProfile .

jdx:hasJob a rdfs:Property ;
    rdfs:label "Has Job Description"@en-US ;
    dct:identifier "jdx:hasJob" ;
    rdfs:comment "Entity referenced is a full description of a job defined and to be offered by the organization being described."@en-US ;
    rdfs:domain schema:Organization ;
    rdfs:isDefinedBy jdx: ;
    rdfs:range jdx:Job .

jdx:hasJobDescription a rdfs:Property ;
    rdfs:label "Has Job Description"@en-US ;
    dct:identifier "jdx:hasJobDescription" ;
    rdfs:comment "Description of a job position generally including the formal job title, duties, purpose, responsibilities, scope, reporting relationships and working conditions along with the knowledge, skills, abilities, education, qualifications, experience and other requirements for performing the job."@en-US ;
    rdfs:domain jdx:Job,
        jdx:JobCompetencyProfile ;
    rdfs:isDefinedBy jdx: ;
    rdfs:range jdx:JobDescription .

jdx:hasJobPosting a rdfs:Property ;
    rdfs:label "Has Job Posting"@en-US ;
    dct:identifier "jdx:hasJobPosting" ;
    rdfs:comment "An online advertisement for filling one or more job position openings that contains information on the employer and the job position based on a job description as well as how and to apply for the job opening and how long the posting is valid for filling the job opening."@en-US ;
    rdfs:domain jdx:Job ;
    rdfs:isDefinedBy jdx: ;
    rdfs:range jdx:JobPosting .

jdx:hasPostingInstructions a rdfs:Property ;
    rdfs:label "Posting Instructions"@en-US ;
    dct:identifier "jdx:hasPostingInstructions" ;
    rdfs:comment "Resource providing instructions for posting a job position opening to a job board or media channel and for submission of applications."@en-US ;
    rdfs:domain jdx:Job,
        jdx:JobPosting ;
    rdfs:isDefinedBy jdx: ;
    rdfs:range jdx:PostingInstructions .

jdx:jobAgreement a rdfs:Property ;
    rdfs:label "Job Agreement"@en-US ;
    dct:identifier "jdx:jobAgreement" ;
    rdfs:comment "Type of employment agreement (e.g. \"employee\", \"contract-to-hire\", \"contract\", \"internship\", \"externship\", \"apprenticeship\", \"student\", \"volunteer\", \"under collective bargaining\", \"eligible for overtime\"; select from an existing enumeration of such types."@en-US ;
    rdfs:domain jdx:Job,
        jdx:JobDescription,
        jdx:JobPosting ;
    rdfs:isDefinedBy jdx: ;
    rdfs:range jdx:AnnotatedDefinedTerm ;
    skos:scopeNote "Use a value selected from a controlled vocabulary of employment contract agreements; select from an existing enumeration of such types."@en-US .

jdx:jobImmediateStart a rdfs:Property ;
    rdfs:label "Job Immediate Start"@en-US ;
    dct:identifier "jdx:jobImmediateStart" ;
    rdfs:comment "Indicator as to whether a position is available for an immediate start."@en-US ;
    rdfs:domain jdx:Job,
        jdx:JobPosting ;
    rdfs:isDefinedBy jdx: ;
    rdfs:range xsd:boolean .

jdx:jobOpeningNumber a rdfs:Property ;
    rdfs:label "Job Opening Number"@en-US ;
    dct:identifier "schema:jobOpeningNumber" ;
    rdfs:comment "Number of positions open at this location."@en-US ;
    rdfs:domain schema:Place ;
    rdfs:isDefinedBy jdx: ;
    rdfs:range xsd:float .

jdx:jobSchedule a rdfs:Property ;
    rdfs:label "Job Schedule"@en-US ;
    dct:identifier "jdx:jobSchedule" ;
    rdfs:comment "Schedule of the employment (e.g. \"full-time\", \"part-time\", \"flex-time\", \"hourly\", \"shared-time\"); select from an existing enumeration of such types."@en-US ;
    rdfs:domain jdx:Job,
        jdx:JobPosting ;
    rdfs:isDefinedBy jdx: ;
    rdfs:range jdx:AnnotatedDefinedTerm ;
    skos:scopeNote "Use a value selected from a controlled vocabulary of employment schedule types; select from an existing enumeration of such types."@en-US .

jdx:jobStartDate a rdfs:Property ;
    rdfs:label "Job Start Date"@en-US ;
    dct:identifier "jdx:jobStartDate" ;
    rdfs:comment "Expected date when the employment begins."@en-US ;
    rdfs:domain jdx:Job,
        jdx:JobPosting ;
    rdfs:isDefinedBy jdx: ;
    rdfs:range xsd:date .

jdx:jobTerm a rdfs:Property ;
    rdfs:label "Job Term"@en-US ;
    dct:identifier "jdx:jobTerm" ;
    rdfs:comment "Type of employment term (e.g. \"regular\", \"temporary\", \"seasonal\"); select from an existing enumeration of such types."@en-US ;
    rdfs:domain jdx:Job,
        jdx:JobDescription,
        jdx:JobPosting ;
    rdfs:isDefinedBy jdx: ;
    rdfs:range jdx:AnnotatedDefinedTerm ;
    skos:scopeNote "Use a value selected from a controlled vocabulary of employment term types; select from an existing enumeration of such types."@en-US .

jdx:knowledge a rdfs:Property ;
    rdfs:label "Knowledge"@en-US ;
    dct:description "Frequently treated as an aspect of the notion of \"competency\" along with \"skills\" and \"abilities\"."@en-US ;
    dct:identifier "jdx:knowledge" ;
    rdfs:comment "Body of facts, principles, theories and practices that is related to a field of work or study; select from an existing enumeration of such types."@en-US ;
    rdfs:domain jdx:Job,
        jdx:JobCompetencyProfile,
        jdx:JobDescription,
        jdx:JobPosting ;
    rdfs:isDefinedBy jdx: ;
    rdfs:range jdx:AnnotatedDefinedTerm ;
    rdfs:subPropertyOf jdx:competency ;
    skos:scopeNote "Use a value selected from a controlled vocabulary of knowledge types such as the O*NET knowledge (https://www.onetonline.org/find/descriptor/browse/Knowledge/); encode using the jdx:AnnotatedDefinedTerm entity."@en-US .

jdx:levelCode a rdfs:Property ;
    rdfs:label "Level Code"@en-US ;
    dct:identifier "jdx:levelCode" ;
    rdfs:comment "Level of experience required; select from an existing enumeration of such types."@en-US ;
    rdfs:domain jdx:QualifyingExperience ;
    rdfs:isDefinedBy jdx: ;
    rdfs:range jdx:AnnotatedDefinedTerm ;
    skos:scopeNote "Use a value selected from a controlled vocabulary of experience level types such as the HR Open CareerLevelCodeList.json; encode using the jdx:AnnotatedDefinedTerm entity."@en-US .

jdx:minimumCredential a rdfs:Property ;
    rdfs:label "Minimum Credential"@en-US ;
    dct:identifier "jdx:minimumCredential" ;
    rdfs:comment "Description of the minimum credential needed for the position or occupation."@en-US ;
    rdfs:domain jdx:Condition,
        jdx:Job,
        jdx:JobDescription,
        jdx:JobPosting ;
    rdfs:isDefinedBy jdx: ;
    rdfs:range jdx:Credential .

jdx:minimumEducation a rdfs:Property ;
    rdfs:label "Minimum Education"@en-US ;
    dct:identifier "jdx:minimumEducation" ;
    rdfs:comment "Description of the minimum education needed for the position or occupation."@en-US ;
    rdfs:domain jdx:Condition,
        jdx:Job,
        jdx:JobDescription,
        jdx:JobPosting ;
    rdfs:isDefinedBy jdx: ;
    rdfs:range jdx:QualifyingExperience .

jdx:minimumExperience a rdfs:Property ;
    rdfs:label "Minimum Experience"@en-US ;
    dct:identifier "jdx:minimumExperience" ;
    rdfs:comment "Description of the minimum experience needed for the position or occupation."@en-US ;
    rdfs:domain jdx:Condition,
        jdx:Job,
        jdx:JobDescription,
        jdx:JobPosting ;
    rdfs:isDefinedBy jdx: ;
    rdfs:range jdx:QualifyingExperience .

jdx:payCycleInterval a rdfs:Property ;
    rdfs:label "Pay Cycle Interval"@en-US ;
    dct:identifier "jdx:payCycleInterval" ;
    rdfs:comment "Pay cycle interval specifies how often the pay cycle occurs or, in other words, how often a person is paid, e.g., \"daily\", \"weekly\", \"monthly\", \"yearly\" etc.; select from an existing enumeration of such types."@en-US ;
    rdfs:domain schema:MonetaryAmount ;
    rdfs:isDefinedBy jdx: ;
    rdfs:range jdx:AnnotatedDefinedTerm ;
    skos:scopeNote "Use a value selected from a controlled vocabulary of pay cycles (e.g., the HR Open PayCycleIntervalCodeList); encode using the jdx:AnnotatedDefinedTerm entity."@en-US .

jdx:physicalActivity a rdfs:Property ;
    rdfs:label "Physical Activity"@en-US ;
    dct:identifier "jdx:physicalActivity" ;
    rdfs:comment "Resource identifying types of physical activity associated with a job; select from an existing enumeration of such types." ;
    rdfs:domain jdx:Job,
        jdx:JobCompetencyProfile,
        jdx:JobDescription,
        jdx:JobPosting ;
    rdfs:isDefinedBy jdx: ;
    rdfs:range jdx:AnnotatedDefinedTerm ;
    skos:scopeNote "Use a value selected from a controlled vocabulary of physical activity types such as \"bending\", \"standing\", \"sitting\"; encode using the jdx:AnnotatedDefinedTerm entity."@en-US .

jdx:physicalRequirement a rdfs:Property ;
    rdfs:label "Physical Requirement"@en-US ;
    dct:identifier "jdx:physicalRequirement" ;
    rdfs:comment "Description of the physical requirements of the job including activities and their associated levels." ;
    rdfs:domain jdx:Job,
        jdx:JobDescription,
        jdx:JobPosting ;
    rdfs:isDefinedBy jdx: ;
    rdfs:range rdf:langString .

jdx:positionID a rdfs:Property ;
    rdfs:label "Position Identifier"@en-US ;
    dct:identifier "jdx:positionID" ;
    rdfs:comment "Employer's identifier for a particular position."@en-US ;
    rdfs:domain jdx:Job,
        jdx:JobDescription ;
    rdfs:isDefinedBy jdx: ;
    rdfs:range xsd:string ;
    rdfs:subPropertyOf schema:identifier .

jdx:postingEndDate a rdfs:Property ;
    rdfs:label "Posting End Date"@en-US ;
    dct:identifier "jdx:postingEndDate" ;
    rdfs:comment "End date (time) for the posting."@en-US ;
    rdfs:domain jdx:PostingInstructions ;
    rdfs:isDefinedBy jdx: ;
    rdfs:range xsd:dateTime .

jdx:postingID a rdfs:Property ;
    rdfs:label "Job Posting Identifier"@en-US ;
    dct:identifier "jdx:postingID" ;
    rdfs:comment "Employer's identifier for a particular job posting."@en-US ;
    rdfs:domain jdx:Job,
        jdx:JobPosting ;
    rdfs:isDefinedBy jdx: ;
    rdfs:range xsd:string ;
    rdfs:subPropertyOf schema:identifier ;
    skos:scopeNote "For the identifier of the position for this posting, use jdx:positionID."@en-US .

jdx:postingRequestor a rdfs:Property ;
    rdfs:label "Posting Requestor"@en-US ;
    dct:identifier "jdx:postingRequestor" ;
    rdfs:comment "Agent requesting the posting."@en-US ;
    rdfs:domain jdx:Job ;
    rdfs:isDefinedBy jdx: ;
    rdfs:range schema:Organization .

jdx:postingStartDate a rdfs:Property ;
    rdfs:label "Posting Start date"@en-US ;
    dct:identifier "jdx:postingStartDate" ;
    rdfs:comment "Start date (time) for the posting."@en-US ;
    rdfs:domain jdx:PostingInstructions ;
    rdfs:isDefinedBy jdx: ;
    rdfs:range xsd:dateTime .

jdx:preferred a rdfs:Property ;
    rdfs:label "Preferred"@en-US ;
    dct:identifier "jdx:preferred" ;
    rdfs:comment "Whether or not the attribute being annotated has been given priority."@en-US ;
    rdfs:domain jdx:ScaleAnnotation ;
    rdfs:isDefinedBy jdx: ;
    rdfs:range xsd:boolean .

jdx:preferredCondition a rdfs:Property ;
    rdfs:label "Preferred Condition"@en-US ;
    dct:identifier "jdx:preferredCondition" ;
    rdfs:comment "Resource referenced provides the means to make logical asserions about alternative conditions."@en-US ;
    rdfs:domain jdx:Condition ;
    rdfs:isDefinedBy jdx: ;
    rdfs:range jdx:Condition .

jdx:preferredCredential a rdfs:Property ;
    rdfs:label "Preferred Experience"@en-US ;
    dct:identifier "jdx:preferredCredential" ;
    rdfs:comment "Description of the preferred credential needed for the position or occupation."@en-US ;
    rdfs:domain jdx:Condition,
        jdx:Job,
        jdx:JobDescription,
        jdx:JobPosting ;
    rdfs:isDefinedBy jdx: ;
    rdfs:range jdx:Credential .

jdx:preferredEducation a rdfs:Property ;
    rdfs:label "Preferred Education"@en-US ;
    dct:identifier "jdx:preferredEducation" ;
    rdfs:comment "Description of the preferred education or training needed for the position or occupation."@en-US ;
    rdfs:domain jdx:Condition,
        jdx:Job,
        jdx:JobDescription,
        jdx:JobPosting ;
    rdfs:isDefinedBy jdx: ;
    rdfs:range jdx:QualifyingExperience .

jdx:preferredExperience a rdfs:Property ;
    rdfs:label "Preferred Experience"@en-US ;
    dct:identifier "jdx:preferredExperience" ;
    rdfs:comment "Description of the preferred experience needed for the position or occupation."@en-US ;
    rdfs:domain jdx:Condition,
        jdx:Job,
        jdx:JobDescription,
        jdx:JobPosting ;
    rdfs:isDefinedBy jdx: ;
    rdfs:range jdx:QualifyingExperience .

jdx:program a rdfs:Property ;
    rdfs:label "Program of Study."@en-US ;
    dct:identifier "jdx:program" ;
    rdfs:comment "Educational program of study."@en-US ;
    rdfs:domain jdx:Credential,
        jdx:QualifyingExperience ;
    rdfs:isDefinedBy jdx: ;
    rdfs:range xsd:langString .

jdx:programConcentration a rdfs:Property ;
    rdfs:label "Program Concentration"@en-US ;
    dct:identifier "jdx:programConcentration" ;
    rdfs:comment "Focused plan of study within a college or university degree such as a concentration in Aerospace Engineering within an Engineering degree."@en-US ;
    rdfs:domain jdx:Credential,
        jdx:QualifyingExperience ;
    rdfs:isDefinedBy jdx: ;
    rdfs:range xsd:langString .

jdx:provider a rdfs:Property ;
    rdfs:label "Provider"@en-US ;
    dct:identifier "jdx:provider" ;
    rdfs:comment "Agent that provides, publishes, owns or otherwise has the authority to make the resource being described available."@en-US ;
    rdfs:domain jdx:Credential,
        jdx:QualifyingExperience ;
    rdfs:isDefinedBy jdx: ;
    rdfs:range schema:Organization .

jdx:qualificationSummary a rdfs:Property ;
    rdfs:label "Qualification Summary"@en-US ;
    dct:identifier "jdx:qualificationSummary" ;
    rdfs:comment "Summary description of the ideal candidate's qualifications for a position."@en-US ;
    rdfs:domain jdx:Job,
        jdx:JobDescription,
        jdx:JobPosting ;
    rdfs:isDefinedBy jdx: ;
    rdfs:range rdf:langString .

jdx:reportingRelationship a rdfs:Property ;
    rdfs:label "Reporting Relationship"@en-US ;
    dct:identifier "jdx:reportingRelationship" ;
    rdfs:comment "Position(s) to which this position reports and over which this position exercises some degree of authority, control or leadership."@en-US ;
    rdfs:domain jdx:Job,
        jdx:JobDescription,
        jdx:JobPosting ;
    rdfs:isDefinedBy jdx: ;
    rdfs:range rdf:langString .

jdx:required a rdfs:Property ;
    rdfs:label "Required"@en-US ;
    dct:identifier "jdx:required" ;
    rdfs:comment "Whether or not the attribute being annotated is required."@en-US ;
    rdfs:domain jdx:ScaleAnnotation ;
    rdfs:isDefinedBy jdx: ;
    rdfs:range xsd:boolean .

jdx:requiredAssessment a rdfs:Property ;
    rdfs:label "Required Assessment"@en-US ;
    dct:identifier "jdx:requiredAssessment" ;
    rdfs:comment "Resource referenced is an example of a direct, indirect, formative, and summative evaluation or estimation of the nature, ability, or quality of a person's performance or outcome of an action."@en-US ;
    rdfs:domain jdx:Job,
        jdx:JobDescription,
        jdx:JobPosting,
        jdx:ScaleAnnotation ;
    rdfs:isDefinedBy jdx: ;
    rdfs:range jdx:AssessmentProfile .

jdx:requiredAtHiring a rdfs:Property ;
    rdfs:label "Required at Hiring"@en-US ;
    dct:identifier "jdx:requiredAtHiring" ;
    rdfs:comment "Whether or not a particular requirement is expected at the time of hiring or may be subsequently obtained."@en-US ;
    rdfs:domain jdx:ScaleAnnotation ;
    rdfs:isDefinedBy jdx: ;
    rdfs:range xsd:boolean .

jdx:requiredCondition a rdfs:Property ;
    rdfs:label "Required Condition"@en-US ;
    dct:identifier "jdx:requiredCondition" ;
    rdfs:comment "Resource referenced provides the means to make logical assertions that combine resources that in aggregate fulfill education, experience and credential requirements."@en-US ;
    rdfs:domain jdx:Condition,
        jdx:Job,
        jdx:JobDescription,
        jdx:JobPosting ;
    rdfs:isDefinedBy jdx: ;
    rdfs:range jdx:Condition .

jdx:requiredCredential a rdfs:Property ;
    rdfs:label "Required credential"@en-US ;
    dct:identifier "jdx:requiredCredential" ;
    rdfs:comment "Description of the required credential needed for the position or occupation."@en-US ;
    rdfs:domain jdx:Condition,
        jdx:Job,
        jdx:JobDescription,
        jdx:JobPosting ;
    rdfs:isDefinedBy jdx: ;
    rdfs:range jdx:Credential .

jdx:requiredEducation a rdfs:Property ;
    rdfs:label "Required Education"@en-US ;
    dct:identifier "jdx:requiredEducation" ;
    rdfs:comment "Description of the required education or training needed for the position or occupation."@en-US ;
    rdfs:domain jdx:Condition,
        jdx:Job,
        jdx:JobDescription,
        jdx:JobPosting ;
    rdfs:isDefinedBy jdx: ;
    rdfs:range jdx:QualifyingExperience ;
    skos:scopeNote "Specific credential requirements should use jdx:requiredCredential."@en-US .

jdx:requiredExperience a rdfs:Property ;
    rdfs:label "Required Experience"@en-US ;
    dct:identifier "jdx:requiredExperience" ;
    rdfs:comment "Description of the required experience needed for the position or occupation."@en-US ;
    rdfs:domain jdx:Condition,
        jdx:Job,
        jdx:JobDescription,
        jdx:JobPosting ;
    rdfs:isDefinedBy jdx: ;
    rdfs:range jdx:QualifyingExperience .

jdx:responsibility a rdfs:Property ;
    rdfs:label "Responsibility"@en-US ;
    dct:identifier "schema:responsibility" ;
    rdfs:comment "Key work tasks or activities over which this position exercises some degree of authority, control or leadership."@en-US ;
    rdfs:domain jdx:Job,
        jdx:JobDescription,
        jdx:JobPosting ;
    rdfs:isDefinedBy jdx: ;
    rdfs:range jdx:AnnotatedDefinedTerm ;
    skos:scopeNote "Use a value selected from a controlled vocabulary of responsibilities; encode using the jdx:AnnotatedDefinedTerm entity."@en-US .

jdx:riskExposure a rdfs:Property ;
    rdfs:label "Risk Exposure"@en-US ;
    dct:identifier "jdx:riskExposure" ;
    rdfs:comment "Description of any exposure to risks associated with the job including exposure to extreme noise or temperature, dust/particle matter, radiation, chemicals, airborne communicable diseases and bloodborne pathogens."@en-US ;
    rdfs:domain jdx:Job,
        jdx:JobCompetencyProfile,
        jdx:JobDescription,
        jdx:JobPosting ;
    rdfs:isDefinedBy jdx: ;
    rdfs:range rdf:langString .

jdx:riskExposureType a rdfs:Property ;
    rdfs:label "Risk Exposure Type"@en-US ;
    dct:identifier "jdx:riskExposureType" ;
    rdfs:comment "Types or categories of risk exposure associated with the job including exposure to extreme noise or temperature, dust/particle matter, radiation, chemicals, airborne communicable diseases and bloodborne pathogens; select from an existing enumeration of such types."@en-US ;
    rdfs:domain jdx:Job,
        jdx:JobCompetencyProfile,
        jdx:JobDescription,
        jdx:JobPosting ;
    rdfs:isDefinedBy jdx: ;
    rdfs:range jdx:AnnotatedDefinedTerm ;
    skos:scopeNote "Use a value selected from a controlled vocabulary of risk exposure types; encode using the jdx:AnnotatedDefinedTerm entity."@en-US .

jdx:scaleCategory a rdfs:Property ;
    rdfs:label "Scale Category"@en-US ;
    dct:description "Where logically applicable, previously defined scales can be applied to a range of previously defined controlled concepts and competencies."@en-US ;
    dct:identifier "jdx:scaleCategory" ;
    rdfs:comment "Type or category of scale or weighting to be applied to a specific competency (knowledge, skill, ability), task, responsibility, interest etc.; select from an existing enumeration of such types."@en-US ;
    rdfs:domain jdx:ScaleAnnotation ;
    rdfs:isDefinedBy jdx: ;
    rdfs:range jdx:AnnotatedDefinedTerm .

jdx:securityClearanceRequirement a rdfs:Property ;
    rdfs:label "Security Clearance Required"@en-US ;
    dct:identifier "jdx:securityClearanceRequired" ;
    rdfs:comment "Description of any security clearance requirements."@en-US ;
    rdfs:domain jdx:Job,
        jdx:JobDescription,
        jdx:JobPosting ;
    rdfs:isDefinedBy jdx: ;
    rdfs:range rdf:langString .

jdx:sensoryCategory a rdfs:Property ;
    rdfs:label "Sensory Category"@en-US ;
    dct:identifier "jdx:sensoryCategory" ;
    rdfs:comment "Types of sensory functions required for sucessful job performance including hearing and vision; select from an existing enumeration of such types." ;
    rdfs:domain jdx:Job,
        jdx:JobCompetencyProfile,
        jdx:JobDescription,
        jdx:JobPosting ;
    rdfs:isDefinedBy jdx: ;
    rdfs:range jdx:AnnotatedDefinedTerm ;
    skos:scopeNote "Use a value selected from a controlled vocabulary of sensory functions; encode using the jdx:AnnotatedDefinedTerm entity."@en-US .

jdx:sensoryRequirement a rdfs:Property ;
    rdfs:label "Sensory Requirement"@en-US ;
    dct:identifier "jdx:sensoryRequirement" ;
    rdfs:comment "Description of sensory requirements and levels necessary to function on the job including hearing and vision." ;
    rdfs:domain jdx:Job,
        jdx:JobCompetencyProfile,
        jdx:JobDescription,
        jdx:JobPosting ;
    rdfs:isDefinedBy jdx: ;
    rdfs:range rdf:langString .

jdx:shiftSchedule a rdfs:Property ;
    rdfs:label "Shift Schedule"@en-US ;
    dct:identifier "jdx:shiftSchedule" ;
    rdfs:comment "Type of the typical work shift of the job; select from an existing enumeration of such types."@en-US ;
    rdfs:domain jdx:Job,
        jdx:JobPosting ;
    rdfs:isDefinedBy jdx: ;
    rdfs:range jdx:AnnotatedDefinedTerm ;
    skos:scopeNote "Use a value selected from a controlled vocabulary of work shift types (e.g., HR Open Standards ShiftTypeCodeList.json); encode using the jdx:AnnotatedDefinedTerm entity."@en-US .

jdx:skill a rdfs:Property ;
    rdfs:label "Skill"@en-US ;
    dct:description "A skill is the ability to carry out a task with determined results often within a given amount of time, energy, or both. (Wikipedia)"@en-US ;
    dct:identifier "jdx:skill" ;
    rdfs:comment "Ability to apply knowledge and use know-how to complete tasks and solve problems including types or categories of developed proficiency or dexterity in mental operations and physical processes required to fulfill a work role; select from an existing enumeration of such types."@en-US ;
    rdfs:domain jdx:Job,
        jdx:JobCompetencyProfile,
        jdx:JobDescription,
        jdx:JobPosting ;
    rdfs:isDefinedBy jdx: ;
    rdfs:range jdx:AnnotatedDefinedTerm ;
    rdfs:subPropertyOf jdx:competency ;
    skos:scopeNote "Use a value selected from a controlled vocabulary of skill types such as the O*NET skills; encode using the jdx:AnnotatedDefinedTerm entity."@en-US .

jdx:task a rdfs:Property ;
    rdfs:label "Task"@en-US ;
    dct:identifier "jdx:task" ;
    rdfs:comment "Piece or unit of work to be done or undertaken and accomplished within a defined period of time or by a deadline; select from an existing enumeration of such types."@en-US ;
    rdfs:domain jdx:Job,
        jdx:JobCompetencyProfile,
        jdx:JobDescription,
        jdx:JobPosting ;
    rdfs:isDefinedBy jdx: ;
    rdfs:range jdx:AnnotatedDefinedTerm ;
    rdfs:subPropertyOf jdx:competency ;
    skos:scopeNote "Use a value selected from a controlled vocabulary of task types such as O*NET tasks; encode using the jdx:AnnotatedDefinedTerm entity."@en-US .

jdx:technology a rdfs:Property ;
    rdfs:label "Technology"@en-US ;
    dct:identifier "jdx:technology" ;
    rdfs:comment "Tool, application or other form of technology that requires knowledge, skill and ability to use effectively in executing the tasks and responsibilities of the job; select from an existing enumeration of such types."@en-US ;
    rdfs:domain jdx:Job,
        jdx:JobDescription,
        jdx:JobPosting ;
    rdfs:isDefinedBy jdx: ;
    rdfs:range jdx:AnnotatedDefinedTerm ;
    skos:scopeNote "Use a value selected from a controlled vocabulary of technology types such as O*NET technology and tools; encode using the jdx:AnnotatedDefinedTerm entity."@en-US .

jdx:totalJobOpenings a rdfs:Property ;
    rdfs:label "Total Job Openings"@en-US ;
    dct:identifier "jdx:totalJobOpenings" ;
    rdfs:comment "Total number of positions open at all locations."@en-US ;
    rdfs:domain jdx:JobPosting ;
    rdfs:isDefinedBy jdx: ;
    rdfs:range xsd:float .

jdx:travelRequirement a rdfs:Property ;
    rdfs:label "Work Travel Requirements"@en-US ;
    dct:identifier "jdx:travelRequirement" ;
    rdfs:comment "Information about any required travel, systematic or occasional."@en-US ;
    rdfs:domain jdx:Job,
        jdx:JobDescription,
        jdx:JobPosting ;
    rdfs:isDefinedBy jdx: ;
    rdfs:range rdf:langString .

jdx:workActivity a rdfs:Property ;
    rdfs:label "Work Activity"@en-US ;
    dct:identifier "jdx:workActivity"@en-US ;
    rdfs:comment "Purposeful, systematic activity by one or more workers acting on a work objective to reach an intended outcome; select from an existing enumeration of such types."@en-US ;
    rdfs:domain jdx:Job,
        jdx:JobDescription,
        jdx:JobPosting ;
    rdfs:isDefinedBy jdx: ;
    rdfs:range jdx:AnnotatedDefinedTerm ;
    rdfs:subPropertyOf jdx:competency ;
    skos:scopeNote "Use a value selected from a controlled vocabulary of activity types such as the O*NET work activities (https://www.onetonline.org/find/descriptor/browse/Work_Activities/); encode using the jdx:AnnotatedDefinedTerm entity."@en-US .

jdx:workLanguage a rdfs:Property ;
    rdfs:label "Work Language"@en-US ;
    dct:identifier "jdx:workLanguage"@en-US ;
    rdfs:comment "Information on the work languages used for the job. (HR)"@en-US ;
    rdfs:domain jdx:Job,
        jdx:JobDescription,
        jdx:JobPosting ;
    rdfs:isDefinedBy jdx: ;
    rdfs:range xsd:language .

schema:additionalProperty a rdfs:Property ;
    rdfs:label "Additional Property"@en-US ;
    dct:identifier "additionalProperty" ;
    rdfs:comment "Property-value pair representing an additional characteristics of the entitity, e.g. a product feature or another characteristic for which there is no matching property in schema.org."@en-US ;
    rdfs:domain jdx:Job,
        jdx:JobCompetencyProfile,
        jdx:JobDescription,
        jdx:JobPosting,
        schema:Organization ;
    rdfs:isDefinedBy schema: ;
    rdfs:range schema:PostalAddress .

schema:address a rdfs:Property ;
    rdfs:label "Address"@en-US ;
    dct:identifier "schema:address" ;
    rdfs:comment "Physical address of the entity."@en-US ;
    rdfs:domain schema:Organization,
        schema:Place ;
    rdfs:isDefinedBy schema: ;
    rdfs:range schema:PostalAddress .

schema:addressCountry a rdfs:Property ;
    rdfs:label "Address Country"@en-US ;
    dct:identifier "schema:addressCountry" ;
    rdfs:comment "The relevant country of the resource. For example, USA."@en-US ;
    rdfs:domain schema:PostalAddress ;
    rdfs:isDefinedBy schema: ;
    rdfs:range rdf:langString .

schema:addressLocality a rdfs:Property ;
    rdfs:label "City"@en-US ;
    dct:identifier "schema:addressLocality" ;
    rdfs:comment "The locality; e.g., Mountain View, London, Moscow."@en-US ;
    rdfs:domain schema:PostalAddress ;
    rdfs:isDefinedBy schema: ;
    rdfs:range rdf:langString .

schema:addressRegion a rdfs:Property ;
    rdfs:label "Address Region"@en-US ;
    dct:identifier "schema:addressRegion" ;
    rdfs:comment "The region; e.g., CA, TX."@en-US ;
    rdfs:domain schema:PostalAddress ;
    rdfs:isDefinedBy schema: ;
    rdfs:range rdf:langString ;
    skos:scopeNote "The relevant state, province, territory or other subdivision of a nation."@en-US .

schema:baseSalary a rdfs:Property ;
    rdfs:label "Base Salary"@en-US ;
    dct:identifier "schema:baseSalary" ;
    rdfs:comment "Base salary of the job or of an employee in an employee role including minimum and maximum salary and unit value (e.g., hour, day, week, month, or year)."@en-US ;
    rdfs:domain jdx:Job,
        jdx:JobPosting ;
    rdfs:isDefinedBy schema: ;
    rdfs:range schema:MonetaryAmount .

schema:contactPoint a rdfs:Property ;
    rdfs:label "Contact Point"@en-US ;
    dct:identifier "schema:contactPoint" ;
    rdfs:comment "A contact point for a person or organization."@en-US ;
    rdfs:domain schema:Organization ;
    rdfs:isDefinedBy schema: ;
    rdfs:range schema:ContactPoint .

schema:contactType a rdfs:Property ;
    rdfs:label "Contact Type"@en-US ;
    dct:identifier "schema:contactType" ;
    rdfs:comment "Specification of the type of contact point."@en-US ;
    rdfs:domain schema:ContactPoint ;
    rdfs:isDefinedBy schema: ;
    rdfs:range jdx:AnnotatedDefinedTerm ;
    skos:scopeNote "Use a value selected from a controlled vocabulary of contact types; encode using the jdx:AnnotatedDefinedTerm entity."@en-US .

schema:currency a rdfs:Property ;
    rdfs:label "Currency"@en-US ;
    dct:identifier "schema:currency" ;
    rdfs:comment "Currency designation (e.g., USD)."@en-US ;
    rdfs:domain schema:MonetaryAmount,
        schema:MonetaryAmountDistribution ;
    rdfs:isDefinedBy <https://schema.org/> ;
    rdfs:range xsd:string .

schema:dateCreated a rdfs:Property ;
    rdfs:label "Date Created"@en-US ;
    dct:identifier "schema:dateCreated" ;
    rdfs:comment "Date on which the position was created."@en-US ;
    rdfs:domain jdx:Job,
        jdx:JobDescription ;
    rdfs:isDefinedBy schema: ;
    rdfs:range xsd:dateTime .

schema:dateModified a rdfs:Property ;
    rdfs:label "Date Modified"@en-US ;
    dct:identifier "schema:dateModified" ;
    rdfs:comment "Date on which the position was modified."@en-US ;
    rdfs:domain jdx:Job,
        jdx:JobDescription ;
    rdfs:isDefinedBy schema: ;
    rdfs:range xsd:dateTime .

schema:datePosted a rdfs:Property ;
    rdfs:label "Date Posted"@en-US ;
    dct:identifier "schema:datePosted" ;
    rdfs:comment "Date of posting by a channel."@en-US ;
    rdfs:domain jdx:JobPosting ;
    rdfs:isDefinedBy schema: ;
    rdfs:range xsd:dateTime .

schema:department a rdfs:Property ;
    rdfs:label "Department"@en-US ;
    dct:identifier "schema:department" ;
    rdfs:comment "Relationship between an organization and a department of that organization."@en-US ;
    rdfs:domain schema:Organization ;
    rdfs:isDefinedBy schema: ;
    rdfs:range schema:Organization .

schema:description a rdfs:Property ;
    rdfs:label "Description"@en-US ;
    dct:identifier "schema:description" ;
    rdfs:comment "A description of the item."@en-US ;
    rdfs:domain jdx:AnnotatedDefinedTerm,
        jdx:AssessmentProfile,
        jdx:Credential,
        jdx:Job,
        jdx:JobCompetencyProfile,
        jdx:JobDescription,
        jdx:JobPosting,
        jdx:QualifyingExperience,
        jdx:ScaleAnnotation,
        schema:ContactPoint,
        schema:DefinedTermSet,
        schema:MonetaryAmount,
        schema:Organization ;
    rdfs:isDefinedBy <https://schema.org/> ;
    rdfs:range rdf:langString ;
    skos:scopeNote "Some online job boards and other services (e.g., Google Jobs) require the general description of a JobPosting to be HTML tagged; in such instances, use the jdx:formattedDescription property instead of the schema:description."@en-US .

schema:duns a rdfs:Property ;
    rdfs:label "DUNS"@en-US ;
    dct:identifier "schema:duns" ;
    rdfs:comment "Dun & Bradstreet DUNS number for identifying an organization or business person."@en-US ;
    rdfs:domain schema:Organization ;
    rdfs:isDefinedBy <https://schema.org/> ;
    rdfs:range xsd:string .

schema:duration a rdfs:Property ;
    rdfs:label "Duration"@en-US ;
    dct:identifier "schema:duration" ;
    rdfs:comment "Duration of the item (movie, audio recording, event, etc.) in ISO 8601 date format."@en-US ;
    rdfs:domain jdx:Credential,
        jdx:QualifyingExperience,
        schema:MonetaryAmountDistribution ;
    rdfs:isDefinedBy <https://schema.org/> ;
    rdfs:range xsd:string .

schema:email a rdfs:Property ;
    rdfs:label "Email Address"@en-US ;
    dct:identifier "schema:email" ;
    rdfs:comment "Email address of an organization or person."@en-US ;
    rdfs:domain schema:ContactPoint,
        schema:Organization ;
    rdfs:isDefinedBy <https://schema.org/> ;
    rdfs:range xsd:string .

schema:estimatedSalary a rdfs:Property ;
    rdfs:label "Estimated Salary"@en-US ;
    dct:description "The estimated salary is usually computed by outside organizations and therefore the hiring organization is not bound to this estimated salary."@en-US ;
    dct:identifier "schema:estimatedSalary" ;
    rdfs:comment "Description of the estimated salary for a job posting based on a variety of variables including, but not limited to industry, job title, and location."@en-US ;
    rdfs:domain jdx:Job ;
    rdfs:isDefinedBy <https://schema.org/> ;
    rdfs:range schema:MonetaryAmountDistribution .

schema:faxNumber a rdfs:Property ;
    rdfs:label "Fax Number"@en-US ;
    dct:identifier "schema:faxNumber" ;
    rdfs:comment "Fax number of an organization or person."@en-US ;
    rdfs:domain schema:ContactPoint,
        schema:Organization,
        schema:Place ;
    rdfs:isDefinedBy <https://schema.org/> ;
    rdfs:range xsd:string .

schema:geo a rdfs:Property ;
    rdfs:label "Geo Coordinates"@en-US ;
    dct:identifier "schema:geo" ;
    rdfs:comment "The geo coordinates of the place."@en-US ;
    rdfs:domain schema:Organization,
        schema:Place ;
    rdfs:isDefinedBy <https://schema.org/> ;
    rdfs:range schema:GeoCoordinates .

schema:hiringOrganization a rdfs:Property ;
    rdfs:label "Hiring Organization"@en-US ;
    dct:identifier "schema:hiringOrganization" ;
    rdfs:comment "Organization offering the job position."@en-US ;
    rdfs:domain jdx:Job,
        jdx:JobDescription,
        jdx:JobPosting ;
    rdfs:isDefinedBy <https://schema.org/> ;
    rdfs:range schema:Organization .

schema:inDefinedTermSet a rdfs:Property ;
    rdfs:label "In Defined Term Set"@en-US ;
    dct:identifier "schema:inDefinedTermSet" ;
    rdfs:comment "A defined term set that contains this term."@en-US ;
    rdfs:domain jdx:AnnotatedDefinedTerm ;
    rdfs:isDefinedBy <https://schema.org/> ;
    rdfs:range schema:DefinedTermSet .

schema:inLanguage a rdfs:Property ;
    rdfs:label "In Language"@en-US ;
    dct:identifier "schema:inLanguage" ;
    rdfs:comment "The language of the content or performance or used in an action."@en-US ;
    rdfs:domain jdx:Credential,
        jdx:Job,
        jdx:JobCompetencyProfile,
        jdx:JobDescription,
        jdx:JobPosting,
        jdx:QualifyingExperience ;
    rdfs:isDefinedBy <https://schema.org/> ;
    rdfs:range xsd:language .

schema:incentiveCompensation a rdfs:Property ;
    rdfs:label "Incentive Compensation"@en-US ;
    dct:identifier "schema:incentiveCompensation" ;
    rdfs:comment "Description of bonus and commission compensation aspects of the job."@en-US ;
    rdfs:domain jdx:Job,
        jdx:JobDescription,
        jdx:JobPosting ;
    rdfs:isDefinedBy <https://schema.org/> ;
    rdfs:range rdf:langString .

schema:industry a rdfs:Property ;
    rdfs:label "Industry"@en-US ;
    dct:identifier "schema:industry" ;
    rdfs:comment "Description of the most critical economic or work activities performed (e.g. software development, electronic manufacturing, motor vehicle production, or diagnostic and therapeutic services)."@en-US ;
    rdfs:domain jdx:Job,
        jdx:JobDescription,
        jdx:JobPosting,
        schema:Organization ;
    rdfs:isDefinedBy <https://schema.org/> ;
    rdfs:range rdf:langString ;
    skos:scopeNote "NOTE: The industry description expected here is a brief narrative of the most critical economic or work activities performed. To identify a formal industry code, such as NAICS in the U.S., use the industryCode property."@en-US .

schema:isicV4 a rdfs:Property ;
    rdfs:label "SIC Code"@en-US ;
    dct:identifier "schema:isicV4" ;
    rdfs:comment "International Standard of Industrial Classification of All Economic Activities (ISIC), Revision 4 code for a particular organization, business person, or place."@en-US ;
    rdfs:domain schema:Organization ;
    rdfs:isDefinedBy <https://schema.org/> ;
    rdfs:range xsd:string .

schema:jobBenefit a rdfs:Property ;
    rdfs:label "Job Benefit"@en-US ;
    dct:identifier "schema:jobBenefit" ;
    rdfs:comment "Description of benefits associated with the job (e.g., \"employee discount\", \"health insurance\", \"401K plan\"); select from an existing enumeration of such types."@en-US ;
    rdfs:domain jdx:Job,
        jdx:JobPosting ;
    rdfs:isDefinedBy <https://schema.org/> ;
    rdfs:range rdf:langString ;
    skos:scopeNote "Use a value selected from a controlled vocabulary of benefit types; select from an existing enumeration of such types."@en-US .

schema:jobLocation a rdfs:Property ;
    rdfs:label "Job Location Type"@en-US ;
    dct:identifier "schema:jobLocation" ;
    rdfs:comment "Typically single geographic location where the work is performed."@en-US ;
    rdfs:domain jdx:Job,
        jdx:JobDescription,
        jdx:JobPosting,
        schema:Organization ;
    rdfs:isDefinedBy <https://schema.org/> ;
    rdfs:range schema:Place .

schema:jobLocationType a rdfs:Property ;
    rdfs:label "Job Location Type"@en-US ;
    dct:identifier "schema:jobLocationType" ;
    rdfs:comment "A description of the job location (e.g., TELECOMMUTE for telecommute jobs)."@en-US ;
    rdfs:domain jdx:Job,
        jdx:JobDescription,
        jdx:JobPosting ;
    rdfs:isDefinedBy <https://schema.org/> ;
    rdfs:range rdf:langString .

schema:latitude a rdfs:Property ;
    rdfs:label "Latitude"@en-US ;
    dct:identifier "schema:latitude" ;
    rdfs:comment "Latitude of a location. For example 37.42242."@en-US ;
    rdfs:domain schema:GeoCoordinates ;
    rdfs:isDefinedBy <https://schema.org/> ;
    rdfs:range xsd:string .

schema:legalName a rdfs:Property ;
    rdfs:label "Legal Name"@en-US ;
    dct:identifier "schema:legalName" ;
    rdfs:comment "The official name of the organization, e.g. the registered company name."@en-US ;
    rdfs:domain schema:Organization ;
    rdfs:isDefinedBy <https://schema.org/> ;
    rdfs:range rdf:langString ;
    rdfs:subPropertyOf schema:name .

schema:leiCode a rdfs:Property ;
    rdfs:label "LEI Code"@en-US ;
    dct:identifier "schema:leiCode" ;
    rdfs:comment "An organization identifier that uniquely identifies a legal entity as defined in ISO 17442."@en-US ;
    rdfs:domain schema:Organization ;
    rdfs:isDefinedBy <https://schema.org/> ;
    rdfs:range xsd:string .

schema:logo a rdfs:Property ;
    rdfs:label "Logo"@en-US ;
    dct:identifier "schema:logo" ;
    rdfs:comment "An associated logo."@en-US ;
    rdfs:domain schema:Organization ;
    rdfs:isDefinedBy <https://schema.org/> ;
    rdfs:range xsd:anyURI .

schema:longitude a rdfs:Property ;
    rdfs:label "Longitude"@en-US ;
    dct:identifier "schema:longitude" ;
    rdfs:comment "Longitude of a location. For example -122.08585."@en-US ;
    rdfs:domain schema:GeoCoordinates ;
    rdfs:isDefinedBy <https://schema.org/> ;
    rdfs:range xsd:string .

schema:maxValue a rdfs:Property ;
    rdfs:label "Maximum Value"@en-US ;
    dct:identifier "schema:maxValue" ;
    rdfs:comment "The upper value of some characteristic or property."@en-US ;
    rdfs:domain schema:MonetaryAmount,
        schema:QuantitativeValue ;
    rdfs:isDefinedBy <https://schema.org/> ;
    rdfs:range xsd:float .

schema:median a rdfs:Property ;
    rdfs:label "Median"@en-US ;
    dct:identifier "schema:median" ;
    rdfs:comment "The median value."@en-US ;
    rdfs:domain schema:MonetaryAmountDistribution ;
    rdfs:isDefinedBy <https://schema.org/> ;
    rdfs:range xsd:float .

schema:minValue a rdfs:Property ;
    rdfs:label "Minimum Value"@en-US ;
    dct:identifier "schema:minValue" ;
    rdfs:comment "The lower value of some characteristic or property."@en-US ;
    rdfs:domain schema:MonetaryAmount,
        schema:QuantitativeValue ;
    rdfs:isDefinedBy <https://schema.org/> ;
    rdfs:range xsd:float .

schema:naics a rdfs:Property ;
    rdfs:label "NAICS"@en-US ;
    dct:identifier "schema:naics" ;
    rdfs:comment "The North American Industry Classification System (NAICS) code for a particular organization or business person."@en-US ;
    rdfs:domain schema:Organization ;
    rdfs:isDefinedBy <https://schema.org/> ;
    rdfs:range xsd:string ;
    rdfs:subPropertyOf jdx:industryCode ;
    owl:equivalentProperty ceterms:naics .

schema:numberOfEmployees a rdfs:Property ;
    rdfs:label "Number of Employees"@en-US ;
    dct:identifier "schema:numberOfEmployees" ;
    rdfs:comment "Number of employees in the hiring organization."@en-US ;
    rdfs:domain schema:Organization ;
    rdfs:isDefinedBy <https://schema.org/> ;
    rdfs:range xsd:integer .

schema:occupationCategory a rdfs:Property ;
    rdfs:label "Occupation Category"@en-US ;
    dct:identifier "occupationCategory" ;
    rdfs:comment "Category of the relevant occupation of the job used in the country of employment; select from an existing enumeration of such types."@en-US ;
    rdfs:domain jdx:Credential,
        jdx:Job,
        jdx:QualifyingExperience ;
    rdfs:isDefinedBy <https://schema.org/> ;
    rdfs:range jdx:AnnotatedDefinedTerm ;
    skos:scopeNote "Use a value selected from a controlled vocabulary of occupation categories such as the Standard Occupational Classification (SOC); encode using the jdx:AnnotatedDefinedTerm entity."@en-US .

schema:parentOrganization a rdfs:Property ;
    rdfs:label "Parent Organization"@en-US ;
    dct:identifier "schema:parentOrganization" ;
    rdfs:comment "The larger organization that this organization is a subOrganization of, if any."@en-US ;
    rdfs:domain schema:Organization ;
    rdfs:isDefinedBy <https://schema.org/> ;
    rdfs:range schema:Organization .

schema:percentile10 a rdfs:Property ;
    rdfs:label "10th Percentile"@en-US ;
    dct:identifier "schema:Percentile10" ;
    rdfs:comment "The 10th percentile value."@en-US ;
    rdfs:domain schema:MonetaryAmountDistribution ;
    rdfs:isDefinedBy <https://schema.org/> ;
    rdfs:range xsd:float .

schema:percentile25 a rdfs:Property ;
    rdfs:label "25th Percentile"@en-US ;
    dct:identifier "schema:Percentile25" ;
    rdfs:comment "The 25th percentile value."@en-US ;
    rdfs:domain schema:MonetaryAmountDistribution ;
    rdfs:isDefinedBy <https://schema.org/> ;
    rdfs:range xsd:float .

schema:percentile75 a rdfs:Property ;
    rdfs:label "75th Percentile"@en-US ;
    dct:identifier "schema:Percentile75" ;
    rdfs:comment "The 75th percentile value."@en-US ;
    rdfs:domain schema:MonetaryAmountDistribution ;
    rdfs:isDefinedBy <https://schema.org/> ;
    rdfs:range xsd:float .

schema:percentile90 a rdfs:Property ;
    rdfs:label "90th Percentile"@en-US ;
    dct:identifier "schema:Percentile90" ;
    rdfs:comment "The 90th percentile value."@en-US ;
    rdfs:domain schema:MonetaryAmountDistribution ;
    rdfs:isDefinedBy <https://schema.org/> ;
    rdfs:range xsd:float .

schema:postalCode a rdfs:Property ;
    rdfs:label "Postal Code"@en-US ;
    dct:identifier "schema:postalCode" ;
    rdfs:comment "Postal code; for example, 94043."@en-US ;
    rdfs:domain schema:PostalAddress ;
    rdfs:isDefinedBy <https://schema.org/> ;
    rdfs:range xsd:string .

schema:propertyID a rdfs:Property ;
    rdfs:label "Property Identifier"@en-US ;
    dct:identifier "schema:propertyID" ;
    rdfs:comment "URL indicating the type of the property and pointing to an external vocabulary."@en-US ;
    rdfs:domain schema:PropertyValue ;
    rdfs:isDefinedBy <https://schema.org/> ;
    rdfs:range xsd:string .

schema:sameAs a rdfs:Property ;
    rdfs:label "Same As"@en-US ;
    dct:identifier "schema:sameAs" ;
    rdfs:comment "URL of a reference Web page that unambiguously indicates the item's identity. E.g. the URL of the item's Wikipedia page, Wikidata entry, or official website."@en-US ;
    rdfs:domain schema:Organization ;
    rdfs:isDefinedBy <https://schema.org/> ;
    rdfs:range xsd:anyURI .

schema:specialCommitment a rdfs:Property ;
    rdfs:label "Special Commitment"@en-US ;
    dct:identifier "schema:specialCommitment" ;
    rdfs:comment "Any special commitments associated with this job posting (e.g. low-income, native American, ex-offenders, military commit) along with any special exclusions (e.g. criminal records)."@en-US ;
    rdfs:domain jdx:Job,
        jdx:JobPosting ;
    rdfs:isDefinedBy <https://schema.org/> ;
    rdfs:range rdf:langString .

schema:streetAddress a rdfs:Property ;
    rdfs:label "Street Address"@en-US ;
    dct:identifier "schema:streetAddress" ;
    rdfs:comment "Street address; for example, \"1600 Amphitheatre Pkwy\"."@en-US ;
    rdfs:domain schema:PostalAddress ;
    rdfs:isDefinedBy <https://schema.org/> ;
    rdfs:range rdf:langString .

schema:subOrganization a rdfs:Property ;
    rdfs:label "Sub-Organization"@en-US ;
    dct:identifier "schema:subOrganization" ;
    rdfs:comment "A relationship between two organizations where the first includes the second, e.g., as a subsidiary."@en-US ;
    rdfs:domain schema:Organization ;
    rdfs:isDefinedBy <https://schema.org/> ;
    rdfs:range schema:Organization .

schema:telephone a rdfs:Property ;
    rdfs:label "Telephone"@en-US ;
    dct:identifier "schema:telephone" ;
    rdfs:comment "The telephone number of an organization or person."@en-US ;
    rdfs:domain schema:ContactPoint,
        schema:Organization,
        schema:Place ;
    rdfs:isDefinedBy <https://schema.org/> ;
    rdfs:range xsd:string .

schema:termCode a rdfs:Property ;
    rdfs:label "Term Code"@en-US ;
    dct:identifier "schema:termCode" ;
    rdfs:comment "A code that identifies this DefinedTerm within a DefinedTermSet."@en-US ;
    rdfs:domain jdx:AnnotatedDefinedTerm ;
    rdfs:isDefinedBy <https://schema.org/> ;
    rdfs:range xsd:string .

schema:title a rdfs:Property ;
    rdfs:label "Title"@en-US ;
    dct:identifier "schema:title" ;
    rdfs:comment "The title of the job."@en-US ;
    rdfs:domain jdx:Job,
        jdx:JobCompetencyProfile,
        jdx:JobDescription,
        jdx:JobPosting ;
    rdfs:isDefinedBy <https://schema.org/> ;
    rdfs:range rdf:langString .

schema:unitText a rdfs:Property ;
    rdfs:label "Unit Text"@en-US ;
    dct:identifier "schema:unitText" ;
    rdfs:comment "Unit of measurement on which values for schema:MonetaryAmount or schema:QuantitativeValue are based; select from an existing enumeration of such types."@en-US ;
    rdfs:domain schema:MonetaryAmount,
        schema:QuantitativeValue ;
    rdfs:isDefinedBy <https://schema.org/> ;
    rdfs:range xsd:string ;
    skos:scopeNote "On schema:MonetaryAmount, Google Jobs recommends using \"HOUR\", \"DAY\", \"WEEK\", \"MONTH\", \"YEAR\"; these values also appear in HR Open's PayCycleIntervalCodeList.json"@en-US .

schema:url a rdfs:Property ;
    rdfs:label "URL"@en-US ;
    dct:identifier "schema:url" ;
    rdfs:comment "URL of the item."@en-US ;
    rdfs:domain schema:DefinedTermSet,
        schema:Organization ;
    rdfs:isDefinedBy <https://schema.org/> ;
    rdfs:range schema:URL .

schema:validFrom a rdfs:Property ;
    rdfs:label "Valid Through"@en-US ;
    dct:identifier "schema:validFrom" ;
    rdfs:comment "The date from which the job posting is valid in ISO 8601 format; for example, \"2017-02-24\" or \"2017-02-24T19:33:17+00:00\"."@en-US ;
    rdfs:domain jdx:JobPosting ;
    rdfs:isDefinedBy <https://schema.org/> ;
    rdfs:range xsd:dateTime .

schema:validThrough a rdfs:Property ;
    rdfs:label "Valid Through"@en-US ;
    dct:description: "The date when the job posting will expire in ISO 8601 format. For example, \"2017-02-24\" or \"2017-02-24T19:33:17+00:00\" (Google) ."@en-US ;
    dct:identifier "schema:validThrough" ;
    rdfs:comment "The date after which the item is not valid. For example the end of an offer, salary period, or a period of opening hours."@en-US ;
    rdfs:domain jdx:JobPosting ;
    rdfs:isDefinedBy <https://schema.org/> ;
    rdfs:range xsd:dateTime .

schema:value a rdfs:Property ;
    rdfs:label "Value"@en-US ;
    dct:identifier "schema:value" ;
    rdfs:comment "Value of the quantitative value or property value node."@en-US ;
    rdfs:domain schema:MonetaryAmount,
        schema:PropertyValue,
        schema:QuantitativeValue ;
    rdfs:isDefinedBy <https://schema.org/> ;
    rdfs:range xsd:string .

schema:workHours a rdfs:Property ;
    rdfs:label "Work Hours"@en-US ;
    dct:identifier "schema:workHours" ;
    rdfs:comment "Typical working hours for this job; e.g. \"1st shift\", \"night shift\", \"8am-5pm\"."@en-US ;
    rdfs:domain jdx:Job,
        jdx:JobDescription,
        jdx:JobPosting ;
    rdfs:isDefinedBy <https://schema.org/> ;
    rdfs:range rdf:langString .

jdx:industryCode a rdfs:Property ;
    rdfs:label "Industry Code"@en-US ;
    dct:identifier "schema:industryCode" ;
    rdfs:comment "Code from a controlled vocabulary of industry types identifying the primary economic activity of an establishment defined as a single physical location where business is conducted or where services or industrial operations are performed."@en-US ;
    rdfs:domain jdx:Job,
        jdx:JobDescription,
        jdx:JobPosting,
        schema:Organization ;
    rdfs:isDefinedBy jdx: ;
    rdfs:range jdx:AnnotatedDefinedTerm ;
    skos:scopeNote "NOTE: In a JDX job description, there my be multiple levels and locations for an organization identified and each may have different industry codes based on the kinds of work performed at those locations; the NAICS industry code here in JDX applies SOLELY to the location where the work of the job being described will be performed."@en-US,
        "NOTE: Use a value selected from a controlled vocabulary of industry types used in the country where the job is located; e.g., NAICS in the U.S. and ESCO in the European Union; encode using the jdx:AnnotatedDefinedTerm entity."@en-US .

schema:name a rdfs:Property ;
    rdfs:label "Name"@en-US ;
    dct:identifier "schema:name" ;
    rdfs:comment "The name of the item."@en-US ;
    rdfs:domain jdx:AnnotatedDefinedTerm,
        jdx:JobCompetencyProfile,
        jdx:JobDescription,
        jdx:JobPosting,
        schema:ContactPoint,
        schema:DefinedTermSet,
        schema:GeoCoordinates,
        schema:Organization,
        schema:Place,
        schema:PostalAddress ;
    rdfs:isDefinedBy <https://schema.org/> ;
    rdfs:range rdf:langString ;
    skos:scopeNote "NOTE: For the name of the hiring organization, use the subproperty legalName."@en-US .

schema:identifier a rdfs:Property ;
    rdfs:label "Position Identifier"@en-US ;
    dct:identifier "schema:identifier" ;
    rdfs:comment "The identifier property represents any kind of identifier for any kind of Thing, such as ISBNs, GTIN codes, UUIDs etc."@en-US ;
    rdfs:domain jdx:Job,
        jdx:JobCompetencyProfile,
        jdx:JobDescription,
        jdx:JobPosting ;
    rdfs:isDefinedBy <https://schema.org/> ;
    rdfs:range schema:PropertyValue ;
    skos:scopeNote "NOTE: Identifier in JDX has a constrained range of schema:PropertyValue. Best practice is to use schema:name property to textually identify the type of identifier, schema:value property to hold the textual value of the identifier, and the schema;properytID for a URI indicating the type of identifier."@en-US,
        "NOTE: JDX defines subproperties called jdx:positionID and jdx:postingID to handle the employer's identifier for a particular position or posting."@en-US .

jdx:competency a rdfs:Property ;
    rdfs:label "Competency"@en-US ;
    dct:identifier "jdx:competency" ;
    rdfs:comment "Observable and measurable knowledge, skills, abilities and personal attributes that contribute to enhanced employee performance of the job; select from an existing enumeration of such types. (HR)"@en-US ;
    rdfs:domain jdx:Job,
        jdx:JobDescription,
        jdx:JobPosting ;
    rdfs:isDefinedBy jdx: ;
    rdfs:range jdx:AnnotatedDefinedTerm ;
    skos:scopeNote "This property has been defined as a super-property for a set of more refined subproperties including knowledge, skills, abilities, attitudes, tasks, and work activities that indicate qualification for the job; encode competencies using the jdx:AnnotatedDefinedTerm entity."@en-US .
