@prefix dct: <http://purl.org/dc/terms/> .
@prefix jdx: <http://purl.org/jdx/terms/> .
@prefix rdf: <http://www.w3.org/1999/02/22-rdf-syntax-ns#> .
@prefix rdfs: <http://www.w3.org/2000/01/rdf-schema#> .
@prefix ceterms: <http://purl.org/ctdl/terms/> .
@prefix asn: <http://purl.org/asn/schema/core/> .
@prefix ceasn: <http://purl.org/ctdlasn/terms/> .
@prefix owl: <http://www.w3.org/2002/07/owl#> .
@prefix schema: <http://schema.org/> .
@prefix skos: <http://www.w3.org/2004/02/skos/core#> .
@prefix vann: <http://purl.org/vocab/vann/> .
@prefix xsd: <http://www.w3.org/2001/XMLSchema#> .

jdx:AnnotatedDefinedTerm a rdfs:Class ;
    dct:identifier "jdx:AnnotatedDefinedTerm"@en-US ;
    rdfs:comment "A word, name, acronym, phrase, defined in a controlled value space (e.g., taxonomy, glossary, dictionary, tag list, and other forms of enumeration)."@en-US ;
    rdfs:isDefinedBy <http://purl.org/jdx/terms/> ;
    rdfs:label "Annotated Defined Term"@en-US ;
    vann:usageNote "Used in the context of JDX to assign terms from occupation, industry and instructional program classifications, skills and abilities, and abstract concepts to JDX entities. Through the class' relationship with the jdx:ScaledAnnotation class, terms can be conditioned through applications of scales for attributes such as importance and frequency."@en-US ;
    vann:usageNote "USE IN PILOT"@en-US .
    
jdx:AssessmentProfile a rdfs:Class ;
    dct:identifier "jdx:AssessmentProfile"@en-US ;
    rdfs:comment "Entity that describes the key characteristics of an assessment administered to candidates for a job."@en-US ;
    rdfs:isDefinedBy <http://purl.org/jdx/terms/> ;
    rdfs:label "Assessment Profile"@en-US ;
    vann:usageNote "USE IN PILOT"@en-US .    

jdx:Condition a rdfs:Class ;
    dct:identifier "jdx:Condition"@en-US ;
    rdfs:comment "Entity providing the means to make logical asserions that combine resources that in aggregate fulfill education, experience and credential requirements."@en-US ;
    rdfs:isDefinedBy <http://purl.org/jdx/terms/> ;
    rdfs:label "Condition"@en-US .    
    
schema:ContactPoint a rdfs:Class ;
    dct:identifier "schema:ContactPoint"@en-US ;
    rdfs:comment "A contact point—e.g., for information about a job opening or interview."@en-US ;
    rdfs:isDefinedBy <http://schema.org/> ;
    rdfs:label "Contact Point"@en-US .
    
jdx:Credential a rdfs:Class ;
    dct:identifier "jdx:Credential"@en-US ;
    rdfs:comment "Entity describing authoritative permission to hold a certain status or to do certain things, e.g. to practice some trade or profession."@en-US ;
    rdfs:isDefinedBy <http://purl.org/jdx/terms/> ;
    rdfs:label "Credential"@en-US .    
  
schema:GeoCoordinates a rdfs:Class ;
    dct:identifier "schema:GeoCoordinates"@en-US ;
    rdfs:comment "Geographic coordinates of a place or event."@en-US ;
    rdfs:isDefinedBy <http://schema.org/> ;
    rdfs:label "Location Geocoordinates"@en-US ;
    vann:usageNote "Use to identify a place using geo coordinates; preferably includes a URI for the location as well as longitude and latitude from a service such as GeoNames (https://www.geonames.org/)."@en-US ;
    vann:usageNote "USE IN PILOT"@en-US .
    
jdx:JobCompetencyProfile a rdfs:Class ;
    dct:identifier "jdx:JobCompetencyProfile"@en-US ;
    rdfs:comment "Entity listing major work tasks, knowledge, skills, and abilities requirements for carrying out those work tasks based on a job analysis that engages subject matter experts in defining and validating the importance, frequency, or other types of weightings of the enumerated competencies."@en-US ;
    rdfs:isDefinedBy <http://purl.org/jdx/terms/> ;
    rdfs:label "Job Competency Profile"@en-US ;
    vann:usageNote "USE IN PILOT"@en-US .
    
jdx:JobDescription a rdfs:Class ;
    dct:identifier "jdx:JobDescription"@en-US ;
    rdfs:comment "Entity providing a statement of a job position generally including the formal job title, duties, purpose, responsibilities, scope, reporting relationships and working conditions along with the knowledge, skills, abilities, education, qualifications, experience and other requirements for performing the job."@en-US ;
    rdfs:isDefinedBy <http://purl.org/jdx/terms/> ;
    rdfs:label "Job Description"@en-US ;
    vann:usageNote "USE IN PILOT"@en-US .
    
jdx:JobMaster a rdfs:Class ;
    dct:identifier "jdx:JobMaster"@en-US ;
    rdfs:comment "Entity used internally as rdfs:domain or \"master\" to which all properties used in JobDescription, JobPosting, and JobCompetencyProfile are applicable. "@en-US ;
    rdfs:isDefinedBy <http://purl.org/jdx/terms/> ;
    rdfs:label "Job Master"@en-US ;
    vann:usageNote "Do NOT use jdx:JobMaster in an entity in any public facing resource."@en-US .
    
jdx:JobPosting a rdfs:Class ;
    dct:identifier "jdx:JobPosting"@en-US ;
    rdfs:comment "Entity describing an on-line advertisement for filling one or more job openings."@en-US ;
    rdfs:isDefinedBy <http://purl.org/jdx/terms/> ;
    rdfs:label "Job Posting"@en-US ;
    vann:usageNote "Entity that contains information on the employer and the job position based on a job description as well as how to apply for the job opening and how long the posting is valid."@en-US ;
    vann:usageNote "USE IN PILOT"@en-US .
            
schema:MonetaryAmountDistribution a rdfs:Class ;
    dct:identifier "schema:MonetaryAmountDistribution"@en-US ;
    rdfs:comment "Statistical distribution of monetary amounts."@en-US ;
    rdfs:isDefinedBy <http://schema.org/> ;
    rdfs:label "Monetary Amount Distribution"@en-US .
        
schema:MonetaryAmount a rdfs:Class ;
    dct:identifier "schema:MonetaryAmount"@en-US ;
    rdfs:comment "A monetary value or range."@en-US ;
    rdfs:isDefinedBy <http://schema.org/> ;
    rdfs:label "Monetary Amount"@en-US ;
    vann:usageNote "This type can be used to describe an amount of money such as $50 USD, or a range as in describing a bank account being suitable for a balance between £1,000 and £1,000,000 GBP, or the value of a salary, etc."@en-US .
    
schema:Organization a rdfs:Class ;
    dct:identifier "schema:Organization"@en-US ;
    rdfs:comment "An organization such as a corporate body, employer, distribution channel provider."@en-US ;
    rdfs:isDefinedBy <http://schema.org/> ;
    rdfs:label "Organization"@en-US .
    
schema:Person a rdfs:Class ;
    dct:identifier "schema:Person"@en-US ;
    rdfs:comment "A human being regarded as an individual. (Oxford)"@en-US ;
    rdfs:isDefinedBy <http://schema.org/> ;
    rdfs:label "Person"@en-US .
    
schema:Place a rdfs:Class ;
    dct:identifier "schema:Place"@en-US ;
    rdfs:comment "A fixed physical location."@en-US ;
    rdfs:isDefinedBy <http://schema.org/> ;
    rdfs:label "Location"@en-US ;
    vann:usageNote "USE IN PILOT"@en-US .
    
schema:PostalAddress a rdfs:Class ;
    dct:identifier "schema:PostalAddress"@en-US ;
    rdfs:comment "The mailing address of an entity."@en-US ;
    rdfs:isDefinedBy <http://schema.org/> ;
    rdfs:label "Postal Address"@en-US ;
    vann:usageNote "USE IN PILOT"@en-US .
    
jdx:PostingInstruction a rdfs:Class ;
    dct:identifier "jdx:PostingInstruction"@en-US ;
    rdfs:comment "An entity providing information about where and how a posting should be communicated."@en-US ;
    rdfs:isDefinedBy <http://purl.org/jdx/terms/> ;
    rdfs:label "Posting Instructions"@en-US ;
    vann:usageNote "A posting channel usually would be a job board or other advertising medium (HR)."@en-US .
        
jdx:QualifyingExperience a rdfs:Class ;
    dct:identifier "jdx:QualifyingExperience"@en-US ;
    rdfs:comment "Entity describing verifiable work, education or training experience supporting a person's qualification to perform the tasks and responsibilities of a position."@en-US ;
    rdfs:isDefinedBy <http://purl.org/jdx/terms/> ;
    rdfs:label "QualifyingExperience"@en-US ;
    vann:usageNote "USE IN PILOT"@en-US .
    
schema:QuantitativeValue a rdfs:Class ;
    dct:identifier "schema:QuantitativeValue"@en-US ;
    rdfs:comment "A point value or interval for product characteristics and other purposes."@en-US ;
    rdfs:isDefinedBy <http://schema.org/> ;
    rdfs:label "Quantitative Value"@en-US .
    
jdx:Rubric a rdfs:Class ;
    dct:identifier "jdx:Rubric"@en-US ;
    rdfs:comment "Resosurce to define assessment criteria and their scoring"@en-US ;
    rdfs:isDefinedBy <http://purl.org/jdx/terms/> ;
    rdfs:label "Rubric"@en-US .
    
jdx:ScaleAnnotation a rdfs:Class ;
    dct:identifier "jdx:ScaleAnnotation"@en-US ;
    rdfs:comment "Resource for identifying and applying a defined scale or rating to another resource."@en-US ;
    rdfs:isDefinedBy <http://purl.org/jdx/terms/> ;
    rdfs:label "Scale Annotation"@en-US ;
    vann:usageNote "Used, for example, when applying an importance scale to a competency identified in an instance of the AnnotatedDefinedTerm class."@en-US ;
    vann:usageNote "USE IN PILOT"@en-US .
              
jdx:ability a rdfs:Property ;
    dct:identifier "jdx:ability"@en-US ;
    rdfs:comment "An aptitude, capacity or power to act physically, socially, mentally, legally, or morally at a level suitable to the work context;select from an existing enumeration of such types."@en-US ;
    rdfs:isDefinedBy <http://purl.org/jdx/terms/> ;
    rdfs:label "Ability"@en-US ;
    rdfs:subPropertyOf jdx:competency ;
    rdfs:domain jdx:JobMaster  ;
    rdfs:range skos:ConceptScheme  ;
    vann:usageNote "Use a value selected from a controlled vocabulary of ability types such as the O*NET cognitive, sensory, psychomotor and physical abilities; encode using the jdx:AnnotatedDefinedTerm entity."@en-US;
    vann:usageNote "USE IN PILOT"@en-US .
    
jdx:acquiredInternally a rdfs:Property ;
    dct:identifier "jdx:acquiredInternally"@en-US ;
    rdfs:comment "Whether or not a requirement in a poosting may be acquired post-hire."@en-US ;
    rdfs:isDefinedBy <http://purl.org/jdx/terms/> ;
    rdfs:label "Acquired Internally"@en-US ;
    rdfs:domain jdx:ScaleAnnotation ;
    rdfs:range xsd:boolean .     
    
jdx:acquisitionDifficulty a rdfs:Property ;
    dct:identifier "jdx:acquisitionDifficulty"@en-US ;
    rdfs:comment "A rating or score representing the difficulty of the particular entity to acquire."@en-US ;
    rdfs:isDefinedBy <http://purl.org/jdx/terms/> ;
    rdfs:label "Acquisition Difficulty"@en-US ;
    rdfs:domain jdx:ScaleAnnotation  ;
    rdfs:range xsd:float  ;
    vann:usageNote "The scale may be applied to any appropriate controlled voabulary concept such as knowledge, skill, and ability as identified in the associated jdx:AnnotationDefinedTerm."@en-US ;
    vann:usageNote "USE IN PILOT"@en-US .
    
schema:address a rdfs:Property ;
    dct:identifier "schema:address"@en-US ;
    rdfs:comment "Physical address of the entity."@en-US ;
    rdfs:isDefinedBy <http://schema.org/> ;
    rdfs:label "Address"@en-US ;
    rdfs:domain schema:Place, schema:Organization  ;
    rdfs:range schema:PostalAddress ;
    vann:usageNote "USE IN PILOT"@en-US .
    
schema:addressCountry a rdfs:Property ;
    dct:identifier "schema:addressCountry"@en-US ;
    rdfs:comment "The relavant country of the resource. For example, USA."@en-US ;
    rdfs:isDefinedBy <http://schema.org/> ;
    rdfs:label "Country Code"@en-US ;
    rdfs:domain schema:PostalAddress  ;
    rdfs:range xsd:string ;
    vann:usageNote "USE IN PILOT"@en-US .
    
schema:addressLocality a rdfs:Property ;
    dct:identifier "schema:addressLocality"@en-US ;
    rdfs:comment "The locality; e.g., Mountain View, London, Moscow."@en-US ;
    rdfs:isDefinedBy <http://schema.org/> ;
    rdfs:label "City"@en-US ;
    rdfs:domain schema:PostalAddress ;
    rdfs:range xsd:string ;
    vann:usageNote "USE IN PILOT"@en-US .
    
schema:addressRegion a rdfs:Property ;
    dct:identifier "schema:addressRegion"@en-US ;
    rdfs:comment "The region; e.g., CA, TX."@en-US ;
    rdfs:isDefinedBy <http://schema.org/> ;
    rdfs:label "Address Region"@en-US ;
    rdfs:domain schema:PostalAddress  ;
    rdfs:range xsd:string  ;
    vann:usageNote "The relevant state, province, territory or other subdivision of a nation state."@en-US ;
    vann:usageNote "USE IN PILOT"@en-US .   
    
jdx:alternativeCondition a rdfs:Property ;
    dct:identifier "jdx:alternativeCondition"@en-US ;
    rdfs:label "Alternative Condition"@en-US ;    
    rdfs:comment "Resource referenced provides the means to make logical asserions about alternative conditions."@en-US ;
    rdfs:isDefinedBy <http://purl.org/jdx/terms/> ;
    rdfs:domain jdx:Condition ;
    rdfs:range jdx:Condition ;
    vann:usageNote "USE IN PILOT"@en-US .
        
jdx:alternativeEducation a rdfs:Property ;
    dct:identifier "jdx:alternativeEducation"@en-US ;
    rdfs:label "Alternative Education"@en-US ;    
    rdfs:comment "Description of an alternative education fulfilling requirements for the position or occupation."@en-US ;
    rdfs:isDefinedBy <http://purl.org/jdx/terms/> ;
    rdfs:domain jdx:Condition, jdx:JobMaster, jdx:JobDescription, jdx:jobPosting ;
    rdfs:range jdx:QualifyingExperience ;
    vann:usageNote "USE IN PILOT"@en-US .
    
jdx:alternativeExperience a rdfs:Property ;
    dct:identifier "jdx:alternativeExperience"@en-US ;
    rdfs:label "Alternative Experience"@en-US ;    
    rdfs:comment "Description of an alternative experience fulfilling requirements for the position or occupation."@en-US ;
    rdfs:isDefinedBy <http://purl.org/jdx/terms/> ;
    rdfs:domain jdx:Condition, jdx:JobMaster, jdx:JobDescription, jdx:jobPosting ;
    rdfs:range jdx:QualifyingExperience ;
    vann:usageNote "USE IN PILOT"@en-US .
    
jdx:alternativeCredential a rdfs:Property ;
    dct:identifier "jdx:alternativeCredential"@en-US ;
    rdfs:label "Alternative Credential"@en-US ;    
    rdfs:comment "Description of an alternative credential fulfilling requirements for the position or occupation."@en-US ;
    rdfs:isDefinedBy <http://purl.org/jdx/terms/> ;
    rdfs:domain jdx:Condition, jdx:JobMaster, jdx:JobDescription, jdx:jobPosting ;
    rdfs:range jdx:Credential ;
    vann:usageNote "USE IN PILOT"@en-US .
    
jdx:annotation a rdfs:Property ;
    dct:identifier "jdx:annotation"@en-US ;
    rdfs:comment "Entity providing qualifying notations including application of scales and other weights to concepts and competencies identified through a jdx:AnnotatedDefinedTerm."@en-US ;
    rdfs:isDefinedBy <http://purl.org/jdx/terms/> ;
    rdfs:label "Related Annotation"@en-US ;
    rdfs:domain jdx:AnnnotatedDefinedTerm  ;
    rdfs:range jdx:ScaleAnnotation ;
    vann:usageNote "USE IN PILOT"@en-US .
    
 jdx:annotatedTerm a rdfs:Property ;
    dct:identifier "jdx:annotatedTerm"@en-US ;
    rdfs:comment "The canonical term identified by the AnnotatedDefinedTerm"@en-US ;
    rdfs:isDefinedBy <http://purl.org/jdx/terms/> ;
    rdfs:label "Annotated Term"@en-US ;
    rdfs:domain jdx:ScaleAnnotation, jdx:JobMaster; jdx:CompetencyProfile, jdx:JobDescription, jdx:JobPosting ;
    rdfs:range skos:Concept; ceasn:Competency; asn:Rubric  ;
    vann:usageNote "Use a value selected from a controlled vocabulary of types; likely external encounters with encodings in schema:DefinedTermSet, schema:DefinedTerm, W3C's SKOS, CTDL-ASN and ASN.."@en-US; 
    
jdx:applicationCloseDate a rdfs:Property ;
    dct:identifier "jdx:applicationCloseDate"@en-US ;
    rdfs:comment "Closing date for accepting applications."@en-US ;
    rdfs:isDefinedBy <http://purl.org/jdx/terms/> ;
    rdfs:label "Application Close Data"@en-US ;
    rdfs:domain jdx:PostingInstructions  ;
    rdfs:range xsd:dateTime .
    
jdx:applicationContact a rdfs:Property ;
    dct:identifier "jdx:applicationContact"@en-US ;
    rdfs:comment "Organization or person contact point for the posting."@en-US ;
    rdfs:isDefinedBy <http://purl.org/jdx/terms/> ;
    rdfs:label "Contact Point"@en-US ;
    rdfs:domain jdx:PostingInstruction  ;
    rdfs:range schema:ContactPoint .
    
jdx:applicationInstructions a rdfs:Property ;
    dct:identifier "jdx:applicationInstructions"@en-US ;
    rdfs:comment "Narrative instructions for applying for this position."@en-US ;
    rdfs:isDefinedBy <http://purl.org/jdx/terms/> ;
    rdfs:label "Application Instructions"@en-US ;
    rdfs:domain jdx:PostingInstructions  ;
    rdfs:range rdf:langString .
    
jdx:applicationLocation a rdfs:Property ;
    dct:identifier "jdx:applicationLocation"@en-US ;
    rdfs:comment "Physical location where job applications can be submitted."@en-US ;
    rdfs:isDefinedBy <http://purl.org/jdx/terms/> ;
    rdfs:label "Application Location"@en-US ;
    rdfs:domain jdx:PostingInstruction  ;
    rdfs:range schema:Place .
    
jdx:applicantLocationRequirement a rdfs:Property ;
    dct:identifier "jdx:applicantLocationRequirement"@en-US ;
    rdfs:comment "Geographic location(s) in which employees may be located for remote (telecommuting) jobs."@en-US ;
    rdfs:isDefinedBy <http://purl.org/jdx/terms/> ;
    rdfs:label "Applicant Location Requirement"@en-US ;
    rdfs:domain jdx:PostingInstruction  ;
    rdfs:range schema:GeoCoordinates ;
    vann:usageNote "USE IN PILOT"@en-US .
    
jdx:approvalStatusCode a rdfs:Property ;
    dct:identifier "jdx:approvalStatusCode"@en-US ;
    rdfs:comment "Values that describe the status of an approval process."@en-US ;
    rdfs:isDefinedBy <http://purl.org/jdx/terms/> ;
    rdfs:label "Approval Status Code"@en-US ;
    rdfs:domain jdx:JobMaster, jdx:JobDescription  ;
    rdfs:range skos:Concept  ;
    vann:usageNote "Use a value selected from a controlled vocabulary of assessment method types such as the HR Open Standards ApprovalStatusCodeList.json; encode using the jdx:AnnotatedDefinedTerm entity."@en-US.
        
jdx:areaAssessed a rdfs:Property ;
    dct:identifier "jdx:areaAssessed"@en-US ;
    rdfs:label "Area Assessed"@en-US ;    
    rdfs:comment "Description of the area or domain to be assessed."@en-US ;
    rdfs:isDefinedBy <http://purl.org/jdx/terms/> ;
    rdfs:domain jdx:AssessmentProfile ;
    rdfs:range rdf:langString .
        
jdx:assessment a rdfs:Property ;
    dct:identifier "jdx:assessment"@en-US ;
    rdfs:comment " Resource comprised of a direct, indirect, formative, and summative evaluation or estimation of the nature, ability, or quality of a person's performance or outcome of an action."@en-US ;
    rdfs:isDefinedBy <http://purl.org/jdx/terms/> ;
    rdfs:label "Assessment"@en-US ;
    rdfs:domain jdx:QualifyingExperience, jdx:Credential ;
    rdfs:range ceterms:Assessment ;
    vann:usageNote "USE IN PILOT"@en-US .
    
jdx:assessmentExample a rdfs:Property ;
    dct:identifier "jdx:assessmentExample"@en-US ;
    rdfs:comment "Resource describing an example assessment."@en-US ;
    rdfs:isDefinedBy <http://purl.org/jdx/terms/> ;
    rdfs:label "Assessment Example"@en-US ;
    rdfs:domain jdx:ScaleAnnotation ;
    rdfs:range xsd:anyURI ;
    vann:usageNote "USE IN PILOT"@en-US . 
 
jdx:assessmentRubric a rdfs:Property ;
    dct:identifier "jdx:assessmentRubric"@en-US ;
    rdfs:comment "Resource provided as assessment rubric for the annotated defined term ."@en-US ;
    rdfs:isDefinedBy <http://purl.org/jdx/terms/> ;
    rdfs:label "Assessment Ribric"@en-US ;
    rdfs:domain jdx:ScaleAnnotation ;
    rdfs:range xsd:anyURI ;
    vann:usageNote "USE IN PILOT"@en-US .
 
jdx:assessmentMethod a rdfs:Property ;
    dct:identifier "jdx:assessmentMethod"@en-US ;
    rdfs:comment "Type of method used to conduct an assessment; select from an existing enumeration of such types."@en-US ;
    rdfs:isDefinedBy <http://purl.org/jdx/terms/> ;
    rdfs:label "Assessment Method"@en-US ;
    rdfs:domain jdx:ScaleAnnotation, jdx:AssessmentProfile  ;
    rdfs:range skos:Concept  ;
    vann:usageNote "Use a value selected from a controlled vocabulary of assessment method types such as the ceterms:AssessmentMethod vocabulary; encode using the jdx:AnnotatedDefinedTerm entity."@en-US;
    vann:usageNote "USE IN PILOT"@en-US .
    
jdx:attitude a rdfs:Property ;
    dct:identifier "jdx:attitude"@en-US ;
    rdfs:comment "Motivators of performance including values, aspirations, and priorities necessary to successful performance of a task or job; select from an existing enumeration of such types."@en-US ;
    rdfs:isDefinedBy <http://purl.org/jdx/terms/> ;
    rdfs:label "Attitude"@en-US ;
    rdfs:domain jdx:JobMaster ;
    rdfs:range skos:Concept ;
    rdfs:subPropertyOf jdx:competency ;
    vann:usageNote "Use a value selected from a controlled vocabulary of attitude types; encode using the jdx:AnnotatedDefinedTerm entity."@en-US ;
    vann:usageNote "USE IN PILOT"@en-US .
    
schema:baseSalary a rdfs:Property ;
    dct:identifier "schema:baseSalary"@en-US ;
    rdfs:comment "The base salary of the job or of an employee in an employee role including minimum and maximum salary and unit value (e.g., hour, day, week, month, or year)."@en-US ;
    rdfs:isDefinedBy <http://schema.org/> ;
    rdfs:label "Base Salary"@en-US ;
    rdfs:domain jdx:JobMaster  ;
    rdfs:range schema:MonetaryAmount ;
    vann:usageNote "USE IN PILOT"@en-US .
    
jdx:careerLevel a rdfs:Property ;
    dct:identifier "jdx:careerLevel"@en-US ;
    rdfs:comment "A code classifying the level of a candidate based on career experience; select from an existing enumeration of such types."@en-US ;
    rdfs:isDefinedBy <http://purl.org/jdx/terms/> ;
    rdfs:label "Career Level"@en-US ;
    rdfs:domain jdx:JobMaster  ;
    rdfs:range skos:Concept  ;
    vann:usageNote "Use a value selected from a controlled vocabulary of career level types (e.g., HR Open Standards CareerLevelCodeList.json); encode using the jdx:AnnotatedDefinedTerm entity."@en-US .
    
jdx:citizenshipRequirement a rdfs:Property ;
    dct:identifier "jdx:citizenshipRequirement"@en-US ;
    rdfs:comment "Required country of the applicant's citizenship."@en-US ;
    rdfs:isDefinedBy <http://purl.org/jdx/terms/> ;
    rdfs:label "Citizenship Requirement"@en-US ;
    rdfs:domain jdx:JobMaster, jdx:JobDescription, jdx:JobPosting ;
    rdfs:range skos:Concept  ;
    vann:usageNote "Use a value selected from a country code list such as the Library of Congress' List of Countries (http://id.loc.gov/vocabulary/countries.html).";  
    vann:usageNote "USE IN PILOT"@en-US .

jdx:competency a rdfs:Property ;
    dct:identifier "jdx:competency"@en-US ;
    rdfs:comment "Combination of observable and measurable knowledge, skills, abilities and personal attributes that contribute to enhanced employee performance; select from an existing enumeration of such types. (HR)"@en-US ;
    rdfs:isDefinedBy <http://purl.org/jdx/terms/> ;
    rdfs:label "Competency"@en-US ;
    rdfs:domain jdx:JobMaster, jdx:JobDescription, jdx:JobPosting  ;
    rdfs:range skos:Concept  ;
    vann:usageNote "This property has been defined as a super-property for a set of more refined subproperties including knowledge, skills, abilities, attitudes, tasks, and work activities that indicate qualification for the job; encode competencyies using the jdx:AnnotatedDefinedTerm entity."@en-US ;
    vann:usageNote "USE IN PILOT"@en-US .
    
jdx:conceptKeyword a rdfs:Property ;
    dct:identifier "jdx:conceptKeyword"@en-US ;
    rdfs:comment "Word or phrase used to refine and describe significant aspects of the entity."@en-US ;
    rdfs:isDefinedBy <http://purl.org/jdx/terms/> ;
    rdfs:label "Concept Keyword"@en-US ;
    rdfs:domain xsd:AssessmentProfile  ;
    rdfs:range rdf:langString .

schema:contactPoint a rdfs:Property ;
    dct:identifier "schema:contactPoint"@en-US ;
    rdfs:comment "A contact point for a person or organization."@en-US ;
    rdfs:isDefinedBy <http://schema.org/> ;
    rdfs:label "Contact Point"@en-US ;
    rdfs:domain schema:Organization, jdx:PostingInstruction ;
    rdfs:range schema:ContactPoint .
    
schema:contactType a rdfs:Property ;
    dct:identifier "schema:contactType"@en-US ;
    rdfs:comment "Specification of the type of contact point."@en-US ;
    rdfs:isDefinedBy <http://schema.org/> ;
    rdfs:label "Contact Type"@en-US ;
    rdfs:domain schema:ContactPoint  ;
    rdfs:range skos:Concept ;
    vann:usageNote "Use a value selected from a controlled vocabulary of contact types; encode using the jdx:AnnotatedDefinedTerm entity."@en-US .
    
jdx:credentialCategory a rdfs:Property ;
    dct:identifier "jdx:credentialCategory"@en-US ;
    rdfs:comment "Type of credential such as badge, certification, bachelor degree; select from an existing enumeration of such types."@en-US ;
    rdfs:isDefinedBy <http://purl.org/jdx/terms/> ;
    rdfs:label "Credential Category"@en-US ;
    rdfs:domain xsd:Credential  ;
    rdfs:range skos:Concept  ;
    owl:equivalentProperty: "http://purl.org/ctdl/terms/credentialType" ;
    vann:usageNote "Use a value selected from a controlled vocabulary of credential types; encode using the jdx:AnnotatedDefinedTerm entity."@en-US .
    
schema:currency a rdfs:Property ;
    dct:identifier "schema:currency"@en-US ;
    rdfs:label "Currency"@en-US ;    
    rdfs:comment "The currency (coded using ISO 4217 ) used for the main salary information in this job posting or for this employee."@en-US ;
    rdfs:isDefinedBy <https://schema.org> ;
    rdfs:domain schema:MonetaryAmountDistribution, schema:MonetaryAmount  ;
    rdfs:range xsd:string ;
    vann:usageNote "USE IN PILOT"@en-US .
    
schema:datePosted a rdfs:Property ;
    dct:identifier "schema:datePosted"@en-US ;
    rdfs:comment "The date of posting by a channel."@en-US ;
    rdfs:isDefinedBy <http://schema.org/> ;
    rdfs:label "Date Posted"@en-US ;
    rdfs:domain jdx:JobPosting  ;
    rdfs:range xsd:dateTime ;
    vann:usageNote "USE IN PILOT"@en-US .
    
schema:department a rdfs:Property ;
    dct:identifier "schema:department"@en-US ;
    rdfs:label "Department"@en-US ;
    rdfs:comment "Relationship between an organization and a department of that organization."@en-US ;
    rdfs:isDefinedBy <http://schema.org/> ;
    rdfs:domain schema:Organization  ;
    rdfs:range schema:Organization .
    
jdx:derivedFrom a rdfs:Property ;
    dct:identifier "jdx:derivedFrom"@en-US ;
    rdfs:label "Derived From"@en-US ;
    rdfs:comment "Identifies a resource from which properties of the resource being described were obtained in whole or in part."@en-US ;
    rdfs:isDefinedBy <http://purl.org/jdx/terms/> ;
    rdfs:domain jdx:JobCompetencyProfile, jdx:JobDescription, jdx:JobPosting  ;
    rdfs:range jdx:JobMaster .
    
schema:description a rdfs:Property ;
    dct:identifier "schema:description"@en-US ;
    rdfs:label "Description"@en-US ;    
    rdfs:comment "A description of the item."@en-US ;
    rdfs:isDefinedBy <https://schema.org> ;
    rdfs:domain jdx:AssessmentProfile, jdx:AnnotatedDefinedTerm, jdx:QualifyingExperience, jdx:JobMaster, jdx:JobCompetencyProfile, jdx:JobDescription, jdx:JobPosting, jdx:Credential, schema:MonetaryAmount, schema:ContactPoint, jdx:ScaleAnnotation,  schema:Organization;
    rdfs:range rdf:langString ;
    vann:usageNote "USE IN PILOT"@en-US .
    
jdx:distributionChannel a rdfs:Property ;
    dct:identifier "jdx:distributionChannel"@en-US ;
    rdfs:label "Distribution Channel"@en-US ;    
    rdfs:comment "Identifies a job board or media channel associated with a job posting."@en-US ;
    rdfs:isDefinedBy <http://purl.org/jdx/terms/> ;
    rdfs:domain jdx:PostingInstructions  ;
    rdfs:range xsd:anyURI .
    
schema:duns a rdfs:Property ;
    dct:identifier "schema:duns"@en-US ;
    rdfs:label "DUNS"@en-US ;    
    rdfs:comment "Dun & Bradstreet DUNS number for identifying an organization or business person."@en-US ;
    rdfs:isDefinedBy <https://schema.org> ;
    rdfs:domain schema:Organization  ;
    rdfs:range xsd:string .
    
schema:duration a rdfs:Property ;
    dct:identifier "schema:duration"@en-US ;
    rdfs:label "Duration"@en-US ;    
    rdfs:comment "Duration of the item (movie, audio recording, event, etc.) in ISO 8601 date format."@en-US ;
    rdfs:isDefinedBy <https://schema.org> ;
    rdfs:domain schema:MonetaryValueDistribution, jdx:QualifyingExperience, jdx:Credential ;
    rdfs:range xsd:string .
    
jdx:educationLevel a rdfs:Property ;
    dct:identifier "schema:educationLevel"@en-US ;
    rdfs:label "Education Level"@en-US ;    
    rdfs:comment "A word or phrase identifying the location of the person in terms of his or her progression through an education or training context; select from an existing enumeration of such types."@en-US ;
    rdfs:isDefinedBy <http://purl.org/jdx/terms/> ;
    rdfs:domain jdx:QualifyingExperience, "jdx:JobMaster", jdx:JobDescription  ;
    rdfs:range skos:Concept  ;
    vann:usageNote "Use a value selected from a controlled vocabulary of education levels such as ceterms:AudienceLevel or HR Open Standards IscedCodeList.json; encode using the jdx:AnnotatedDefinedTerm entity."@en-US .
    
schema:email a rdfs:Property ;
    dct:identifier "schema:email"@en-US ;
    rdfs:label "Email Address"@en-US ;    
    rdfs:comment "Email address of an organization or person."@en-US ;
    rdfs:isDefinedBy <https://schema.org> ;
    rdfs:domain schema:Organization, schema:ContactPoint  ;
    rdfs:range xsd:string .
     
jdx:employerOverview a rdfs:Property ;
    dct:identifier "jdx:employerOverview"@en-US ;
    rdfs:label "Employer Overview"@en-US ;    
    rdfs:comment "Description of the employer, career opportunities and work environment."@en-US ;
    rdfs:isDefinedBy <https://schema.org> ;
    rdfs:domain jdx:JobMaster, jdx:JobPosting  ;
    rdfs:range rdf:langString ;
    vann:usageNote "USE IN PILOT"@en-US .
    
jdx:employmentUnit a rdfs:Property ;
    dct:identifier "jdx:employmentUnit"@en-US ;
    rdfs:label "Employment Unit"@en-US ;    
    rdfs:comment "Department or unit where the employee reports and/or in which the job is to be performed."@en-US ;
    rdfs:isDefinedBy <http://purl.org/jdx/terms/> ;
    rdfs:domain jdx:JobDescription, jdx:JobPosting, jdx:JobMaster ;
    rdfs:range schema:Organization ;
    vann:usageNote "USE IN PILOT"@en-US .
    
jdx:employmentUnitName a rdfs:Property ;
    dct:identifier "jdx:employmentUnitName"@en-US ;
    rdfs:label "Employment Unit Name"@en-US ;    
    rdfs:comment "Name of department or unit where the employee reports and/or in which the job is to be performed."@en-US ;
    rdfs:isDefinedBy <http://purl.org/jdx/terms/> ;
    rdfs:domain schema:Organization ;
    rdfs:range rdf:langString ;
    rdfs:subPropertyOf schema:name ;
    vann:usageNote "USE IN PILOT"@en-US .
    
jdx:equivalentExperience a rdfs:Property ;
    dct:identifier "jdx:equivalentEperience"@en-US ;
    rdfs:label "Equivalent Experience"@en-US ;    
    rdfs:comment "Description of equivalent experience for the position or occupation."@en-US ;
    rdfs:isDefinedBy <http://purl.org/jdx/terms/> ;
    rdfs:domain jdx:Condition, jdx:JobMaster, jdx:JobDescription, jdx:jobPosting ;
    rdfs:range jdx:QualifyingExperience ;
    vann:usageNote "USE IN PILOT"@en-US .
    
jdx:equivalentCredential a rdfs:Property ;
    dct:identifier "jdx:equivalentCredential"@en-US ;
    rdfs:label "Equivalent Credential"@en-US ;    
    rdfs:comment "Description of an equivalent credential for the position or occupation."@en-US ;
    rdfs:isDefinedBy <http://purl.org/jdx/terms/> ;
    rdfs:domain jdx:Condition, jdx:JobMaster, jdx:JobDescription, jdx:jobPosting ;
    rdfs:range jdx:Credential ;
    vann:usageNote "USE IN PILOT"@en-US .
    
jdx:equivalentEducation a rdfs:Property ;
    dct:identifier "jdx:equivalentEducation"@en-US ;
    rdfs:label "Equivalent Education"@en-US ;    
    rdfs:comment "Description of equivalent education for the position or occupation."@en-US ;
    rdfs:isDefinedBy <http://purl.org/jdx/terms/> ;
    rdfs:domain jdx:Condition, jdx:JobMaster, jdx:JobDescription, jdx:jobPosting ;
    rdfs:range jdx:QualifyingExperience ;
    vann:usageNote "USE IN PILOT"@en-US .
    
jdx:expectedStartDate a rdfs:Property ;
    dct:identifier "jdx:expectedStartDate"@en-US ;
    rdfs:label "ExpectedStart Date"@en-US ;    
    rdfs:comment "Expected date when the employment begins."@en-US ;
    rdfs:isDefinedBy <http://purl.org/jdx/terms/> ;
    rdfs:domain jdx:JobMaster, jdx:JobPosting ;
    rdfs:range xsd:date ;
    vann:usageNote "USE IN PILOT"@en-US .
    
schema:estimatedSalary a rdfs:Property ;
    dct:identifier "schema:estimatedSalary"@en-US ;
    rdfs:label "Estimated Salary"@en-US ;    
    rdfs:comment "A property describing the estimated salary for a job posting based on a variety of variables including, but not limited to industry, job title, and location."@en-US ;
    dct:description "The estimated salary is usually computed by outside organizations and therefore the hiring organization is not bound to this estimated salary."@en-US ;
    rdfs:isDefinedBy <https://schema.org> ;
    rdfs:domain jdx:JobMaster, jdx:JobDescription, jdx:JobPosting  ;
    rdfs:range schema:MonetaryAmountDistribution .
    
jdx:evidence a rdfs:Property ;
    dct:identifier "jdx:evidence"@en-US ;
    rdfs:label "Evidence"@en-US ;    
    rdfs:comment "The referenced artifact or performance confirming or supporting an assertion."@en-US ;
    rdfs:isDefinedBy <http://purl.org/jdx/terms/> ;
    rdfs:domain jdx:QualifyingExperience, jdx:Credential  ;
    rdfs:range xsd:anyUri .
    
jdx:evidenceCategory a rdfs:Property ;
    dct:identifier "jdx:evidenceType"@en-US ;
    rdfs:label "EvidenceType"@en-US ;    
    rdfs:comment "The type of referenced artifact, exam or performance confirming or supporting an assertion; select from an existing enumeration of such types."@en-US ;
    rdfs:isDefinedBy <http://purl.org/jdx/terms/> ;
    rdfs:domain jdx:QualifyingExperience, jdx:Credential, jdx:ScaleAnnotation, jdx:AssessmentProfile ;
    rdfs:range skos:Concept  ;
    vann:usageNote "Use a value selected from a controlled vocabulary of evidence types; encode using the jdx:AnnotatedDefinedTerm entity."@en-US ;
    vann:usageNote "USE IN PILOT"@en-US .
    
jdx:experienceCategory a rdfs:Property ;
    dct:identifier "jdx:experienceCategory"@en-US ;
    rdfs:label "Experience Category"@en-US ;    
    rdfs:comment "Category of experience needed for the position or Occupation; select from an existing enumeration of such types."@en-US ;
    rdfs:isDefinedBy <http://purl.org/jdx/terms/> ;
    rdfs:domain jdx:QualifyingExperience, jdx:JobMaster, jdx:JobDescription; 
    rdfs:range skos:Concept ;
    vann:usageNote "Use a value selected from a controlled vocabulary of experience types including, but not limited to, \"Education Experience\", \"Training Experience\", \"Work Experience\" and it's subtypes \"Apprenticeship\" and \"Traineeship\"; encode using the jdx:AnnotatedDefinedTerm entity."@en-US .
    
schema:faxNumber a rdfs:Property ;
    dct:identifier "schema:faxNumber"@en-US ;
    rdfs:label "Fax Number"@en-US ;    
    rdfs:comment "The fax number of an organization or person."@en-US ;
    rdfs:isDefinedBy <https://schema.org> ;
    rdfs:domain schema:Place, schema:Organization, schema:ContactPoint  ;
    rdfs:range xsd:string ;
    vann:usageNote "USE IN PILOT"@en-US .
    
jdx:fein a rdfs:Property ;
    dct:identifier "jdx:fein"@en-US ;
    rdfs:label "FEIN"@en-US ;    
    rdfs:comment "Federal Employer Identification Number (FEIN) identifying organizations, persons, states, government agencies, corporations, and companies."@en-US ;
    rdfs:isDefinedBy <http://purl.org/jdx/terms/> ;
    rdfs:domain schema:Organization  ;
    rdfs:range xsd:string  ;
    owl:equivalentProperty: "http://purl.org/ctdl/terms/fein" .
    
jdx:formattedDescription a rdfs:Property ;
    dct:identifier "jdx:formattedDescription"@en-US ;
    rdfs:label "Formatted Description"@en-US ;    
    rdfs:comment "Complete representation of the job, including job responsibilities, qualifications, skills, working hours, education requirements, and experience requirements."@en-US ;
    rdfs:isDefinedBy <http://purl.org/jdx/terms/> ;
    rdfs:domain jdx:JobMaster, jdx:JobPosting, jdx:jobCompetencyProfile, jdx:JobDescription  ;
    vann:usageNote "The description should support HTML or other markup."@en-US ;
    vann:usageNote "Determine datatype encoding 
    rdfs:range rdf:langString .
    
schema:geo a rdfs:Property ;
    dct:identifier "schema:geo"@en-US ;
    rdfs:label "Geo Coordinates"@en-US ;    
    rdfs:comment "The geo coordinates of the place."@en-US ;
    rdfs:isDefinedBy <https://schema.org> ;
    rdfs:domain schema:Organization, schema:Place  ;
    rdfs:range schema:GeoCoordinates ;
    vann:usageNote "USE IN PILOT"@en-US .
       
jdx:hasCompetencyProfile a rdfs:Property ;
    dct:identifier "jdx:hasCompetencyProfile"@en-US ;
    rdfs:label "Has Competency Profile@"@en-US ;    
    rdfs:comment "Listing of the major work tasks, knowledge, skills, and abilities requirements for carrying out those work tasks based on a job analysis that engages subject matter experts in defining and validating the importance, frequency, or other types of weightings of the enumerated competencies."@en-US ;
    rdfs:isDefinedBy <http://purl.org/jdx/terms/> ;
    rdfs:domain schema:Organization, jdx:JobDescription  ;
    rdfs:range jdx:JobCompetencyProfile  .
    
jdx:hasJobDescription a rdfs:Property ;
    dct:identifier "jdx:hasJobDescription"@en-US ;
    rdfs:label "Has Job Description"@en-US ;    
    rdfs:comment "Description of a job position generally including the formal job title, duties, purpose, responsibilities, scope, reporting relationships and working conditions along with the knowledge, skills, abilities, education, qualifications, experience and other requirements for performing the job."@en-US ;
    rdfs:isDefinedBy <http://purl.org/jdx/terms/> ;
    rdfs:domain schema:Organization, jdx:JobCompetencyProfile, jdx:JobPosting ;
    rdfs:range jdx:JobDescription .
    
jdx:hasJobPosting a rdfs:Property ;
    dct:identifier "jdx:hasJobPosting"@en-US ;
    rdfs:label "Has Job Posting"@en-US ;    
    rdfs:comment "An online advertisement for filling one or more job position openings that contains information on the employer and the job position based on a job description as well as how and to apply for the job opening and how long the posting is valid for filling the job opening."@en-US ;
    rdfs:isDefinedBy <http://purl.org/jdx/terms/> ;
    rdfs:domain schema:Organization  ;
    rdfs:range jdx:JobPosting .
    
jdx:hasPostingInstructions a rdfs:Property ;
    dct:identifier "jdx:hasPostingInstructions"@en-US ;
    rdfs:label "Posting Instructions"@en-US ;    
    rdfs:comment "Entity providing instructions for posting a job position opening to a job board or media channel and for submission of applications."@en-US ;
    rdfs:isDefinedBy <http://purl.org/jdx/terms/> ;
    rdfs:domain jdx:JobMaster, jdx:jobPosting ;
    rdfs:range jdx:PostingInstructions .
    
schema:hiringOrganization a rdfs:Property ;
    dct:identifier "schema:hiringOrganization"@en-US ;
    rdfs:label "Hiring Organization"@en-US ;    
    rdfs:comment "Organization making the job offer."@en-US ;
    rdfs:isDefinedBy <https://schema.org> ;
    rdfs:domain jdx:JobMaster, jdx:JobDescription, jdx:JobPosting ;
    rdfs:range schema:Organization ;
    vann:usageNote "USE IN PILOT"@en-US .
    
 schema:identifier a rdfs:Property ;
    dct:identifier "schema:identifier"@en-US ;
    rdfs:label "Position Identifier"@en-US ;    
    rdfs:comment "The identifier for the position that may be used externally in an advertisement."@en-US ;
    rdfs:isDefinedBy <http://purl.org/jdx/terms/> ;
    rdfs:domain jdx:jobMaster, jdx:JobCompetencyProfile, jdx:JobDescription, jdx:JobPosting ;
    rdfs:range xsd:string ;
    vann:usageNote "USE IN PILOT"@en-US .
    
jdx:immediateStartIndicator a rdfs:Property ;
    dct:identifier "jdx:immediateStartIndicator"@en-US ;
    rdfs:label "Immediate Start Indicator"@en-US ;    
    rdfs:comment "An indicator as to whether a position is available for an immediate start."@en-US ;
    rdfs:isDefinedBy <http://purl.org/jdx/terms/> ;
    rdfs:domain jdx:JobMaster, jdx:JobPosting ;
    rdfs:range xsd:boolean .
    
schema:incentiveCompensation a rdfs:Property ;
    dct:identifier "schema:incentiveCompensation"@en-US ;
    rdfs:label "Incentive Compensation"@en-US ;    
    rdfs:comment "Description of bonus and commission compensation aspects of the job."@en-US ;
    rdfs:isDefinedBy <https://schema.org> ;
    rdfs:domain jdx:JobMaster, jdx:JobDescription ; 
    rdfs:range rdf:langString ;
    vann:usageNote "USE IN PILOT"@en-US .
    
schema:inDefinedTermSet a rdfs:Property ;
    dct:identifier "schema:inDefinedTermSet"@en-US ;
    rdfs:label "In Defined Term Set"@en-US ;    
    rdfs:comment "A defined term set that contains this term."@en-US ;
    rdfs:isDefinedBy <https://schema.org> ;
    rdfs:domain jdx:AnnotatedDefinedTerm  ;
    rdfs:range jdx:AnnotatedDefinedTermSet .
    
schema:industry a rdfs:Property ;
    dct:identifier "schema:industryType"@en-US ;
    rdfs:label "Industry"@en-US ;    
    rdfs:comment "Primary economic activity of an establishment defined as a single physical location where business is conducted or where services or industrial operations are performed (for example, a
factory, mill, store, hotel, movie theater, mine, farm, airline terminal, sales office, warehouse, or
central administrative office)."@en-US ;
    rdfs:isDefinedBy <https://schema.org> ;
    rdfs:domain jdx:QualifyingExperience, jdx:Credential, jdx:JobMaster, jdx:JobDescription;
    rdfs:range skos:Concept  ;
    vann:usageNote "Use a value selected from a controlled vocabulary of industry types used in the country where the job is located; e.g., NAICS in the U.S. and ESCO in the European Union; encode using the jdx:AnnotatedDefinedTerm entity."@en-US .
    
schema:inLanguage a rdfs:Property ;
    dct:identifier "schema:inLanguag"@en-US ;
    rdfs:label "In Language"@en-US ;    
    rdfs:comment "The language of the content or performance or used in an action."@en-US ;
    rdfs:isDefinedBy <https://schema.org> ;
    rdfs:domain jdx:JobMaster, jdx:JobCompetencyProfile, jdx:JobDescription, jdx:JobPosting, jdx:QualifyingExperience, jdx:Credential;
    rdfs:range xsd:language  .
    
schema:isicV4 a rdfs:Property ;
    dct:identifier "schema:isicV4"@en-US ;
    rdfs:label "SIC Code"@en-US ;    
    rdfs:comment "International Standard of Industrial Classification of All Economic Activities (ISIC), Revision 4 code for a particular organization, business person, or place."@en-US ;
    rdfs:isDefinedBy <https://schema.org> ;
    rdfs:domain schema:Organization  ;
    rdfs:range xsd:string .
    
jdx:jobAgreementCategory a rdfs:Property ;
    dct:identifier "jdx:jobAgreementCategory"@en-US ;
    rdfs:label "Job Agreement Category"@en-US ;    
    rdfs:comment "Type of employment agreement (e.g. employee, contract, temporary, seasonal, internship, under collectively bargaining, eligible for overtime); select from an existing enumeration of such types."@en-US ;
    rdfs:isDefinedBy <https://schema.org> ;
    rdfs:domain jdx:JobMaster, jdx:JobDescription, jdx:JobPosting  ;
    rdfs:range skos:Concept  ;
    vann:usageNote "Use a value selected from a controlled vocabulary of employment contract agreements; select from an existing enumeration of such types."@en-US ;
    vann:usageNote "USE IN PILOT"@en-US .
    
schema:jobBenefit a rdfs:Property ;
    dct:identifier "schema:jobBenefit"@en-US ;
    rdfs:label "Job Benefit"@en-US ;    
    rdfs:comment "Description of benefits associated with the job."@en-US ;
    rdfs:isDefinedBy <https://schema.org> ;
    rdfs:domain jdx:JobMaster, jdx:JobPosting ;
    rdfs:range rdf:langString ;
    vann:usageNote "USE IN PILOT"@en-US .
    
schema:jobLocation a rdfs:Property ;
    dct:identifier "schema:jobLocation"@en-US ;
    rdfs:label "Job Location"@en-US ;    
    rdfs:comment "A (typically single) geographic location associated with the job position."@en-US ;
    rdfs:isDefinedBy <https://schema.org> ;
    rdfs:domain jdx:JobMaster, jdx:JobDescription, jdx:JobCompetencyProfile, jdx:JobPosting ;
    rdfs:range schema:Place ;
    vann:usageNote "USE IN PILOT"@en-US .
    
schema:jobLocationType a rdfs:Property ;
    dct:identifier "schema:jobLocationType"@en-US ;
    rdfs:label "Job Location Type"@en-US ;    
    rdfs:comment "A description of the job location (e.g., TELECOMMUTE for telecommute jobs)."@en-US ;
    rdfs:isDefinedBy <https://schema.org> ;
    rdfs:domain jdx:jobCompetencyProfile, jdx:jobDescription, jdx:jobPosting ;
    rdfs:range rdf:langString ;
    vann:usageNote "USE IN PILOT"@en-US .
    
schema:jobOpeningNumber a rdfs:Property ;
    dct:identifier "schema:jobOpeningNumber"@en-US ;
    rdfs:label "Job Opening Number"@en-US ;    
    rdfs:comment "Number of positions open for this job."@en-US ;
    rdfs:isDefinedBy <https://schema.org> ;
    rdfs:domain jdx:jobPosting ;
    rdfs:range xsd:float .
    
jdx:jobScheduleCategory a rdfs:Property ;
    dct:identifier "jdx:jobScheduleCategory"@en-US ;
    rdfs:label "Job Schedule Category"@en-US ;    
    rdfs:comment "Type of employment schedule (e.g. full-time, part-time, flex-time, shared-time); select from an existing enumeration of such types."@en-US ;
    rdfs:isDefinedBy <https://schema.org> ;
    rdfs:domain jdx:JobMaster, jdx:JobDescription, jdx:JobPosting  ;
    rdfs:range skos:Concept  ;
    vann:usageNote "Use a value selected from a controlled vocabulary of employment schedule types; select from an existing enumeration of such types."@en-US ;
    vann:usageNote "USE IN PILOT"@en-US .
    
jdx:jobTermCategory a rdfs:Property ;
    dct:identifier "jdx:jobTermCategory"@en-US ;
    rdfs:label "Job Term Category"@en-US ;    
    rdfs:comment "Type of employment term (e.g. regular, temporary, seasonal); select from an existing enumeration of such types."@en-US ;
    rdfs:isDefinedBy <https://schema.org> ;
    rdfs:domain jdx:JobMaster, jdx:JobDescription, jdx:JobPosting  ;
    rdfs:range skos:Concept  ;
    vann:usageNote "Use a value selected from a controlled vocabulary of employment term types; select from an existing enumeration of such types."@en-US ;
    vann:usageNote "USE IN PILOT"@en-US .
    
jdx:knowledge a rdfs:Property ;
    dct:identifier "jdx:knowledge"@en-US ;
    rdfs:label "Knowledge"@en-US ;    
    rdfs:comment "Body of facts, principles, theories and practices that is related to a field of work or study; select from an existing enumeration of such types."@en-US ;
    dct:description "Frequently treated as an aspect of the notion of \"competency\" along with skills and abilities."@en-US ;
    rdfs:isDefinedBy <http://purl.org/jdx/terms/> ;
    rdfs:domain jdx:JobMaster, jdx:JobCompetencyProfile, jdx:JobDescription, jdx:JobOpening, jdx:JobPosting ; 
    rdfs:range skos:Concept  ;
    rdfs:subPropertyOf jdx:competency ;
    vann:usageNote "Use a value selected from a controlled vocabulary of knowledge types such as the O*NET knowledge (https://www.onetonline.org/find/descriptor/browse/Knowledge/); encode using the jdx:AnnotatedDefinedTerm entity."@en-US ;
    vann:usageNote "USE IN PILOT"@en-US .
    
schema:latitude a rdfs:Property ;
    dct:identifier "schema:latitude"@en-US ;
    rdfs:label "Latitude"@en-US ;    
    rdfs:comment "The latitude of a location. For example 37.42242."@en-US ;
    rdfs:isDefinedBy <https://schema.org> ;
    rdfs:domain schema:GeoCoordinates  ;
    rdfs:range xsd:string ;
    vann:usageNote "USE IN PILOT"@en-US .
    
schema:legalName a rdfs:Property ;
    dct:identifier "schema:legalName"@en-US ;
    rdfs:label "Legal Name"@en-US ;    
    rdfs:comment "The official name of the organization, e.g. the registered company name."@en-US ;
    rdfs:isDefinedBy <https://schema.org> ;
    rdfs:domain schema:Organization  ;
    rdfs:range rdf:langString .
    
schema:leiCode a rdfs:Property ;
    dct:identifier "schema:leiCode"@en-US ;
    rdfs:label "LEI Code"@en-US ;    
    rdfs:comment "An organization identifier that uniquely identifies a legal entity as defined in ISO 17442."@en-US ;
    rdfs:isDefinedBy <https://schema.org> ;
    rdfs:domain schema:Organization  ;
    rdfs:range xsd:string .
    
jdx:levelCode a rdfs:Property ;
    dct:identifier "jdx:levelCode"@en-US ;
    rdfs:label "Level Code"@en-US ;    
    rdfs:comment "Level of experience required; select from an existing enumeration of such types."@en-US ;
    rdfs:isDefinedBy <http://purl.org/jdx/terms/> ;
    rdfs:domain jdx:QualifyingExperience  ;
    rdfs:range skos:Concept  ;
    vann:usageNote "Use a value selected from a controlled vocabulary of experience level types; encode using the jdx:AnnotatedDefinedTerm entity."@en-US .
    
schema:logo a rdfs:Property ;
    dct:identifier "schema:logo"@en-US ;
    rdfs:label "Logo"@en-US ;    
    rdfs:comment "An associated logo."@en-US ;
    rdfs:isDefinedBy <https://schema.org> ;
    rdfs:domain schema:Organization ;
    rdfs:range xsd:anyURI .
        
schema:location a rdfs:Property ;
    dct:identifier "schema:location"@en-US ;
    rdfs:label "location"@en-US ;    
    rdfs:comment "The location where the event is happening, an organization is located, or where an action takes place."@en-US ;
    rdfs:isDefinedBy <https://schema.org> ;
    rdfs:domain schema:Organization ;
    rdfs:range schema:Place .
    
schema:longitude a rdfs:Property ;
    dct:identifier "schema:longitude"@en-US ;
    rdfs:label "Longitude"@en-US ;    
    rdfs:comment "The longitude of a location. For example -122.08585."@en-US ;
    rdfs:isDefinedBy <https://schema.org> ;
    rdfs:domain schema:GeoCoordinates  ;
    rdfs:range xsd:string  ;
    vann:usageNote "USE IN PILOT"@en-US .
    
schema:maxValue a rdfs:Property ;
    dct:identifier "schema:maxValue"@en-US ;
    rdfs:label "Maximum Value"@en-US ;    
    rdfs:comment "The upper value of some characteristic or property."@en-US ;
    rdfs:isDefinedBy <https://schema.org> ;
    rdfs:domain schema:QuantitativeValue; schema:MonetaryAmount  ;
    rdfs:range xsd:float ;
    vann:usageNote "USE IN PILOT"@en-US .
    
schema:median a rdfs:Property ;
    dct:identifier "schema:median"@en-US ;
    rdfs:label "Median"@en-US ;    
    rdfs:comment "The median value."@en-US ;
    rdfs:isDefinedBy <https://schema.org> ;
    rdfs:domain schema:MonetaryAmountDistribution  ;
    rdfs:range xsd:float .
        
jdx:minimumEducation a rdfs:Property ;
    dct:identifier "jdx:minimumEducation"@en-US ;
    rdfs:label "Minimum Education"@en-US ;    
    rdfs:comment "Description of the minimum education needed for the position or occupation."@en-US ;
    rdfs:isDefinedBy <http://purl.org/jdx/terms/> ;
    rdfs:domain jdx:Condition, jdx:JobMaster, jdx:JobDescription, jdx:jobPosting ;
    rdfs:range jdx:QualifyingExperience ;
    vann:usageNote "USE IN PILOT"@en-US .
    
jdx:minimumExperience a rdfs:Property ;
    dct:identifier "jdx:minimumExperience"@en-US ;
    rdfs:label "Minimum Experience"@en-US ;    
    rdfs:comment "Description of the minimum experience needed for the position or occupation."@en-US ;
    rdfs:isDefinedBy <http://purl.org/jdx/terms/> ;
    rdfs:domain jdx:Condition, jdx:JobMaster, jdx:JobDescription, jdx:jobPosting ;
    rdfs:range jdx:QualifyingExperience ;
    vann:usageNote "USE IN PILOT"@en-US .
    
jdx:minimumCredential a rdfs:Property ;
    dct:identifier "jdx:minimumCredential"@en-US ;
    rdfs:label "Minimum Credential"@en-US ;    
    rdfs:comment "Description of the minimum credential needed for the position or occupation."@en-US ;
    rdfs:isDefinedBy <http://purl.org/jdx/terms/> ;
    rdfs:domain jdx:Condition, jdx:JobMaster, jdx:JobDescription, jdx:jobPosting ;
    rdfs:range jdx:Credential ;
    vann:usageNote "USE IN PILOT"@en-US .    
    
schema:minValue a rdfs:Property ;
    dct:identifier "schema:minValue"@en-US ;
    rdfs:label "Minimum Value"@en-US ;    
    rdfs:comment "The lower value of some characteristic or property."@en-US ;
    rdfs:isDefinedBy <https://schema.org> ;
    rdfs:domain schema:QuantitativeValue; schema:MonetaryAmount  ;
    rdfs:range xsd:float ;
    vann:usageNote "USE IN PILOT"@en-US .
    
schema:naics a rdfs:Property ;
    dct:identifier "schema:naics"@en-US ;
    rdfs:label "NAICS"@en-US ;    
    rdfs:comment "The North American Industry Classification System (NAICS) code for a particular organization or business person."@en-US ;
    rdfs:isDefinedBy <https://schema.org> ;
    rdfs:domain schema:Organization  ;
    rdfs:range xsd:string  ;
    owl:equivalentProperty ceterms:naics .
    
schema:name a rdfs:Property ;
    dct:identifier "schema:name"@en-US ;
    rdfs:label "Name"@en-US ;    
    rdfs:comment "The name of the item."@en-US ;
    rdfs:isDefinedBy <https://schema.org> ;
    rdfs:domain jdx:JobCompetencyProfile, jdx:JobDescription, jdx:JobPosting, jdx:AnnotatedDefinedTerm, schema:Place, schema:PostalAddress, schema:ContactPoint, schema:Organization, schema:GeoCoordinates ;
    rdfs:range rdf:langString ;
    vann:usageNote "USE IN PILOT"@en-US .
    
schema:numberOfEmployees a rdfs:Property ;
    dct:identifier "schema:numberOfEmployees"@en-US ;
    rdfs:label "Number of Employees"@en-US ;    
    rdfs:comment "The number of employees in an organization e.g. business."@en-US ;
    rdfs:isDefinedBy <https://schema.org> ;
    rdfs:domain schema:Organization  ;
    rdfs:range xsd:integer .
    
schema:occupationCategory a rdfs:Property ;
    dct:identifier "occupationCategory"@en-US ;
    rdfs:label "Occupation Category"@en-US ;    
    rdfs:comment "Category or categories of the relevant occupation of the job used in the country of employment; select from an existing enumeration of such types."@en-US ;
    rdfs:isDefinedBy <https://schema.org> ;
    rdfs:domain jdx:JobMaster, jdx:QualifyingExperience, jdx:Credential;
    rdfs:range skos:Concept  ;
    vann:usageNote "Use a value selected from a controlled vocabulary of occupation categories such as the Standard Occupational Classification (SOC); encode using the jdx:AnnotatedDefinedTerm entity."@en-US ;
    vann:usageNote "USE IN PILOT"@en-US .
    
jdx:organization a rdfs:Property ;
    dct:identifier "jdx:organization"@en-US ;
    rdfs:label "Organization"@en-US ;    
    rdfs:comment "Organization that issued or otherwise provided the resource."@en-US ;
    rdfs:isDefinedBy <http://purl.org/jdx/terms/> ;
    rdfs:domain jdx:QualifyingExperience, jdx:Credential  ;
    rdfs:range schema:Organization .
    
schema:parentOrganization a rdfs:Property ;
    dct:identifier "schema:parentOrganization"@en-US ;
    rdfs:label "Parent Organization"@en-US ;    
    rdfs:comment "The larger organization that this organization is a subOrganization of, if any."@en-US ;
    rdfs:isDefinedBy <https://schema.org> ;
    rdfs:domain schema:Organization  ;
    rdfs:range schema:Organization .
    
schema:percentile10 a rdfs:Property ;
    dct:identifier "schema:Percentile10"@en-US ;
    rdfs:label "10th Percentile"@en-US ;    
    rdfs:comment "The 10th percentile value."@en-US ;
    rdfs:isDefinedBy <https://schema.org> ;
    rdfs:domain schema:MonetaryAmoungDistribution ;
    rdfs:range xsd:float .
    
schema:percentile25 a rdfs:Property ;
    dct:identifier "schema:Percentile25"@en-US ;
    rdfs:label "25th Percentile"@en-US ;    
    rdfs:comment "The 25th percentile value."@en-US ;
    rdfs:isDefinedBy <https://schema.org> ;
    rdfs:domain schema:MonetaryAmountDistribution  ;
    rdfs:range xsd:float .
    
schema:percentile75 a rdfs:Property ;
    dct:identifier "schema:Percentile75"@en-US ;
    rdfs:label "75th Percentile"@en-US ;    
    rdfs:comment "The 75th percentile value."@en-US ;
    rdfs:isDefinedBy <https://schema.org> ;
    rdfs:domain schema:MonetaryAmountDistribution  ;
    rdfs:range xsd:float .
    
schema:percentile90 a rdfs:Property ;
    dct:identifier "schema:Percentile90"@en-US ;
    rdfs:label "90th Percentile"@en-US ;    
    rdfs:comment "The 90th percentile value."@en-US ;
    rdfs:isDefinedBy <https://schema.org> ;
    rdfs:domain schema:MonetaryAmountDistribution  ;
    rdfs:range xsd:float .
    
jdx:physicalActivityCategory a rdfs:Property ;
    dct:identifier "jdx:physicalActivityCategory"@en-US ;
    rdfs:label "Physical Activity Category"@en-US ;
    rdfs:comment "Resource identifying types of physical activity associated with a job." ;    
    rdfs:isDefinedBy <http://purl.org/jdx/terms/> ;
    rdfs:domain jdx:JobMaster, jdx:jobCompetencyProfile, jdx:JobDescription, jdx:JobPosting ;
    rdfs:range skos:Concept ;
    vann:usageNote "Use a value selected from a controlled vocabulary of physical activity types such as \"bending\", \"standing\", \"sitting\"; encode using the jdx:AnnotatedDefinedTerm entity."@en-US ;
    vann:usageNote "USE IN PILOT"@en-US .
    
jdx:physicalRequirement a rdfs:Property ;
    dct:identifier "jdx:physicalRequirement"@en-US ;
    rdfs:label "Physical Requirement"@en-US ;
    rdfs:comment "Description of the physical requirements of the job including activities and their associated levels." ;     
    rdfs:isDefinedBy <http://purl.org/jdx/terms/> ;
    rdfs:domain jdx:JobMaster, jdx:jobCompetencyProfile, jdx:JobDescription, jdx:JobPosting ;
    rdfs:range rdf:langString ;
    vann:usageNote "USE IN PILOT"@en-US .  
    
schema:postalCode a rdfs:Property ;
    dct:identifier "schema:postalCode"@en-US ;
    rdfs:label "Postal Code"@en-US ;    
    rdfs:comment "The postal code. For example, 94043."@en-US ;
    rdfs:isDefinedBy <https://schema.org> ;
    rdfs:domain schema:PostalAddress  ;
    rdfs:range xsd:string ;
    vann:usageNote "USE IN PILOT"@en-US .
    
jdx:postingEndDate a rdfs:Property ;
    dct:identifier "jdx:postingEndDate"@en-US ;
    rdfs:label "Posting End Date"@en-US ;    
    rdfs:comment "End date (time) for the posting."@en-US ;
    rdfs:isDefinedBy <http://purl.org/jdx/terms/> ;
    rdfs:domain jdx:PostingInstructions  ;
    rdfs:range xsd:dateTime .
    
jdx:postingRequestor a rdfs:Property ;
    dct:identifier "jdx:postingRequestor"@en-US ;
    rdfs:label "Posting Requestor"@en-US ;    
    rdfs:comment "The agent requesting the posting."@en-US ;
    rdfs:isDefinedBy <http://purl.org/jdx/terms/> ;
    rdfs:domain jdx:JobMaster  ;
    rdfs:range schema:Organization .
    
jdx:postingStartDate a rdfs:Property ;
    dct:identifier "jdx:postingStartDate"@en-US ;
    rdfs:label "Posting Start date"@en-US ;    
    rdfs:comment "Start date (time) for the posting."@en-US ;
    rdfs:isDefinedBy <http://purl.org/jdx/terms/> ;
    rdfs:domain jdx:PostingInstructions  ;
    rdfs:range xsd:dateTime .
     
jdx:preferred a rdfs:Property ;
    dct:identifier "jdx:preferred"@en-US ;
    rdfs:label "Preferred"@en-US ;    
    rdfs:comment "Whether or not the attribute being annotated has been given priority."@en-US ;
    rdfs:isDefinedBy <http://purl.org/jdx/terms/> ;
    rdfs:domain schema:ScaleAnnotation  ;
    rdfs:range xsd:boolean ;
    vann:usageNote "USE IN PILOT"@en-US .
    
jdx:preferredEducation a rdfs:Property ;
    dct:identifier "jdx:preferredEducation"@en-US ;
    rdfs:label "Preferred Education"@en-US ;    
    rdfs:comment "Description of the preferred credential needed for the position or occupation."@en-US ;
    rdfs:isDefinedBy <http://purl.org/jdx/terms/> ;
    rdfs:domain jdx:Condition, jdx:JobMaster, jdx:JobDescription, jdx:jobPosting ;
    rdfs:range jdx:QualifyingExperience ;
    vann:usageNote "USE IN PILOT"@en-US .
        
jdx:preferredExperience a rdfs:Property ;
    dct:identifier "jdx:preferredExperience"@en-US ;
    rdfs:label "Preferred Experience"@en-US ;    
    rdfs:comment "Description of the preferred experience needed for the position or occupation."@en-US ;
    rdfs:isDefinedBy <http://purl.org/jdx/terms/> ;
    rdfs:domain jdx:Condition, jdx:JobMaster, jdx:JobDescription, jdx:jobPosting ;
    rdfs:range jdx:QualifyingExperience ;
    vann:usageNote "USE IN PILOT"@en-US .
    
jdx:preferredCredential a rdfs:Property ;
    dct:identifier "jdx:preferredCredential"@en-US ;
    rdfs:label "Preferred Experience"@en-US ;    
    rdfs:comment "Description of the preferred credential needed for the position or occupation."@en-US ;
    rdfs:isDefinedBy <http://purl.org/jdx/terms/> ;
    rdfs:domain jdx:Condition, jdx:JobMaster, jdx:JobDescription, jdx:jobPosting ;
    rdfs:range jdx:Credential ;
    vann:usageNote "USE IN PILOT"@en-US .
    
jdx:program a rdfs:Property ;
    dct:identifier "jdx:program"@en-US ;
    rdfs:label "Program of Study."@en-US ;    
    rdfs:comment "Degree program of study."@en-US ;
    rdfs:isDefinedBy <http://purl.org/jdx/terms/> ;
    rdfs:domain jdx:QualifyingExperience ;
    rdfs:range xsd:langString .
    
jdx:programConcentration a rdfs:Property ;
    dct:identifier "jdx:programConcentration"@en-US ;
    rdfs:label "Program Concentration"@en-US ;    
    rdfs:comment "Focused plan of study within a college or university degree such as a concentration in Aerospace Engineering within an Engineering degree."@en-US ;
    rdfs:isDefinedBy <http://purl.org/jdx/terms/> ;
    rdfs:domain jdx:QualifyingExperience ;
    rdfs:range xsd:langString .
    
jdx:qualificationSummary a rdfs:Property ;
    dct:identifier "jdx:qualificationSummary"@en-US ;
    rdfs:label "Qualification Summary"@en-US ;    
    rdfs:comment "Summary description of the ideal candidate's qualifications for a position."@en-US ;
    rdfs:isDefinedBy <http://purl.org/jdx/terms/> ;
    rdfs:domain jdx:JobOpening  ;
    rdfs:range rdf:langString .
    
jdx:required a rdfs:Property ;
    dct:identifier "jdx:required"@en-US ;
    rdfs:label "Required"@en-US ;    
    rdfs:comment "Whether or not the attribute being annotated is required."@en-US ;
    rdfs:isDefinedBy <http://purl.org/jdx/terms/> ;
    rdfs:domain jdx:ScaleAnnotation ;
    vann:usageNote "USE IN PILOT"@en-US .
    
jdx:requiredAssessment a rdfs:Property ;
    dct:identifier "jdx:requiredAssessment"@en-US ;
    rdfs:label "Required Assessment"@en-US ;    
    rdfs:comment "Assessment of a candidate employees qualifications."@en-US ;
    rdfs:isDefinedBy <http://purl.org/jdx/terms/> ;
    rdfs:domain jdx:ScaleAnnotation; job:master; jobDescription; jdx:JobPosting ;
    rdfs:range jdx:AssessmentProfile .

jdx:requiredAtHiring a rdfs:Property ;
    dct:identifier "jdx:requiredAtHiring"@en-US ;
    rdfs:label "Required at Hiring"@en-US ;    
    rdfs:comment "Whether or not a particular requirement is expected at the time of hiring or may be subsequently obtained."@en-US ;
    rdfs:isDefinedBy <http://purl.org/jdx/terms/> ;
    rdfs:domain jdx:ScaleAnnotation  ;
    rdfs:range xsd:boolean .
    
jdx:requiredCondition a rdfs:Property ;
    dct:identifier "jdx:requiredCondition"@en-US ;
    rdfs:label "Required Condition"@en-US ;    
    rdfs:comment "Resource referenced provides the means to make logical assertions that combine resources that in aggregate fulfill education, experience and credential requirements."@en-US ;
    rdfs:isDefinedBy <http://purl.org/jdx/terms/> ;
    rdfs:domain jdx:Condition, jdx:JobMaster, jdx:JobDescription, jdx:jobPosting ;
    rdfs:range jdx:Condition ;
    vann:usageNote "See github issue: https://github.com/jobdataexchange/Data-Modeling/issues/12"@en-US 
        
jdx:requiredEducation a rdfs:Property ;
    dct:identifier "jdx:requiredEducation"@en-US ;
    rdfs:label "Required Education"@en-US ;    
    rdfs:comment "Description of the required education needed for the position or occupation - specific credential requirements should use required credential."@en-US ;
    rdfs:isDefinedBy <http://purl.org/jdx/terms/> ;
    rdfs:domain jdx:Condition, jdx:JobMaster, jdx:JobDescription, jdx:jobPosting ;
    rdfs:range jdx:QualifyingExperience ;
    vann:usageNote "USE IN PILOT"@en-US .

jdx:requiredExperience a rdfs:Property ;
    dct:identifier "jdx:requiredExperience"@en-US ;
    rdfs:label "Required Experience"@en-US ;    
    rdfs:comment "Description of the required experience needed for the position or occupation."@en-US ;
    rdfs:isDefinedBy <http://purl.org/jdx/terms/> ;
    rdfs:domain jdx:Condition, jdx:JobMaster, jdx:JobDescription, jdx:jobPosting ;
    rdfs:range jdx:QualifyingExperience ;
    vann:usageNote "USE IN PILOT"@en-US .
    
jdx:requiredCredential a rdfs:Property ;
    dct:identifier "jdx:requiredCredential"@en-US ;
    rdfs:label "Required credential"@en-US ;    
    rdfs:comment "Description of the required credential needed for the position or occupation."@en-US ;
    rdfs:isDefinedBy <http://purl.org/jdx/terms/> ;
    rdfs:domain jdx:Condition, jdx:JobMaster, jdx:JobDescription, jdx:jobPosting ;
    rdfs:range jdx:Credential ;
    vann:usageNote "USE IN PILOT"@en-US .
    
jdx:reportingRelationship a rdfs:Property ;
    dct:identifier "jdx:reportingRelationship"@en-US ;
    rdfs:label "Reporting Relationship"@en-US ;
    rdfs:comment Position(s) to which this position reports and over which this position exercises some degree of authority, control or leadership."@en-US ;     
    rdfs:isDefinedBy <http://purl.org/jdx/terms/> ;
    rdfs:domain jdx:JobMaster, jdx:JobDescription ;
    rdfs:range rdf:langString ;
    vann:usageNote "USE IN PILOT"@en-US .
    
schema:responsibilities a rdfs:Property ;
    dct:identifier "schema:responsibility"@en-US ;
    rdfs:label "Responsibility"@en-US ;    
    rdfs:comment "Key work tasks or activities over which this position exercises some degree of authority, control or leadership."@en-US ;
    rdfs:isDefinedBy <http://purl.org/jdx/terms/> ;
    rdfs:domain jdx:JobMaster, jdx:JobCompetencyProfile, jdx:JobDescription, jdx:JobPosting ; 
    rdfs:range rdf:langString ;
    vann:usageNote "USE IN PILOT"@en-US .
    
jdx:riskExposure a rdfs:Property ;
    dct:identifier "jdx:riskExposure"@en-US ;
    rdfs:label "Risk Exposure"@en-US ;
    rdfs:comment "Description of any exposure to risks associated with the job including exposure to extreme noise or temperature, dust/particle matter, radiation, chemicals, airborne communicable diseases and bloodborne pathogens."@en-US;     
    rdfs:isDefinedBy <http://purl.org/jdx/terms/> ;
    rdfs:domain jdx:JobMaster, jdx:jobCompetencyProfile, jdx:JobDescription, jdx:JobPosting ;
    rdfs:range rdf:langString ;
    vann:usageNote "USE IN PILOT"@en-US .
    
jdx:riskExposureType a rdfs:Property ;
    dct:identifier "jdx:riskExposureType"@en-US ;
    rdfs:label "Risk Exposure Type"@en-US ;
    rdfs:comment "Types or categories of risk exposure associated with the job including exposure to extreme noise or temperature, dust/particle matter, radiation, chemicals, airborne communicable diseases and bloodborne pathogens."@en-US;     
    rdfs:isDefinedBy <http://purl.org/jdx/terms/> ;
    rdfs:domain jdx:JobMaster, jdx:jobCompetencyProfile, jdx:JobDescription, jdx:JobPosting ;
    rdfs:range skos:concept  ;
    vann:usageNote "Use a value selected from a controlled vocabulary of risk exposure types; encode using the jdx:AnnotatedDefinedTerm entity."@en-US ;
    vann:usageNote "USE IN PILOT"@en-US .

schema:sameAs a rdfs:Property ;
    dct:identifier "schema:sameAs"@en-US ;
    rdfs:label "Same As"@en-US ;    
    rdfs:comment "URL of a reference Web page that unambiguously indicates the item's identity. E.g. the URL of the item's Wikipedia page, Wikidata entry, or official website."@en-US ;
    rdfs:isDefinedBy <https://schema.org> ;
    rdfs:domain schema:Organization  ;
    rdfs:range xsd:anyURI .
    
jdx:scaleCategory a rdfs:Property ;
    dct:identifier "jdx:scaleCategory"@en-US ;
    rdfs:label "Scale Category"@en-US ;    
    rdfs:comment "Type or category of scale or weighting to be applied to a specific competency (knowledge, skill, ability), task, responsibility, interest etc.; select from an existing enumeration of such types."@en-US ;
    dct:description "Where logically applicable, previously defined scales can be applied to a range of previously defined controlled concepts and competencies."@en-US ;
    rdfs:isDefinedBy <http://purl.org/jdx/terms/> ;
    rdfs:domain jdx:ScaleAnnontation ;
    rdfs:range skos:concept  ;
    vann:usageNote "Use a value selected from a controlled vocabulary of scale types; encode using the jdx:AnnotatedDefinedTerm entity."@en-US ;
    vann:usageNote "USE IN PILOT"@en-US .
    
jdx:scaleValue a rdfs:Property ;
    dct:identifier "jdx:scaleValue"@en-US ;
    rdfs:label "Scale Value"@en-US ;    
    rdfs:comment "Quantitative value and unit type of the weight, degree, percent, or strength of a recommendation or requirementto a specific competency (knowledge, skill, ability), task, responsibility, interest being annotated."@en-US ;
    rdfs:isDefinedBy <http://purl.org/jdx/terms/> ;
    rdfs:domain jdx:ScaleAnnontation ;
    rdfs:range schema:QuantitativeValue ;
    vann:usageNote "USE IN PILOT"@en-US .
    
jdx:securityClearanceRequirement a rdfs:Property ;
    dct:identifier "jdx:securityClearanceRequired"@en-US ;
    rdfs:comment "Description of any security clearance requirements."@en-US ;
    rdfs:isDefinedBy <http://purl.org/jdx/terms/> ;
    rdfs:label "Security Clearance Required"@en-US ;
    rdfs:domain jdx:JobMaster, jdx:JobDescription, jdx:JobPosting ;
    rdfs:range rdf:langString ;
    vann:usageNote "USE IN PILOT"@en-US .

jdx:sensoryRequirement a rdfs:Property ;
    dct:identifier "jdx:sensoryRequirement"@en-US ;
    rdfs:label "Sensory Requirement"@en-US ;
    rdfs:comment "Description of sensory requirements and levels necessary to function on the job including hearing and vision." ;     
    rdfs:isDefinedBy <http://purl.org/jdx/terms/> ;
    rdfs:domain jdx:JobMaster, jdx:jobCompetencyProfile, jdx:JobDescription, jdx:JobPosting ;
    rdfs:range rdf:langString ;
    vann:usageNote "USE IN PILOT"@en-US .
    
jdx:skill a rdfs:Property ;
    dct:identifier "jdx:skill"@en-US ;
    rdfs:label "Skill"@en-US ;    
    rdfs:comment "Ability to apply knowledge and use know-how to complete tasks and solve problems including types or categories of developed proficiency or dexterity in mental operations and physical processes required to fulfill a work role; select from an existing enumeration of such types."@en-US ;
    dct:description "(Wikipedia) A skill is the ability to carry out a task with determined results often within a given amount of time, energy, or both."@en-US ;
    rdfs:isDefinedBy <http://purl.org/jdx/terms/> ;
    rdfs:domain jdx:JobMaster, jdx:JobCompetencyProfile, jdx:JobDescription, jdx:JobPosting ;
    rdfs:range skos:Concept ;
    rdfs:subPropertyOf jdx:competency ;
    vann:usageNote "Use a value selected from a controlled vocabulary of skill types such as the O*NET skills; encode using the jdx:AnnotatedDefinedTerm entity."@en-US ;
    vann:usageNote "USE IN PILOT"@en-US .
    
schema:specialCommitment a rdfs:Property ;
    dct:identifier "schema:specialCommitment"@en-US ;
    rdfs:label "Special Commitment"@en-US ;    
    rdfs:comment "Any special commitments associated with this job (e.g. low-income, native American, ex-offenders, military commit) along with any special exclusions (e.g. criminal records)."@en-US ;
    rdfs:isDefinedBy <https://schema.org> ;
    rdfs:domain jdx:JobMaster, jdx:JobPosting ;
    rdfs:range rdf:langString ;
    vann:usageNote "USE IN PILOT"@en-US .
    
schema:streetAddress a rdfs:Property ;
    dct:identifier "schema:streetAddress"@en-US ;
    rdfs:label "Street Address"@en-US ;    
    rdfs:comment "The street address. For example, 1600 Amphitheatre Pkwy."@en-US ;
    rdfs:isDefinedBy <https://schema.org> ;
    rdfs:domain schema:PostalAddress  ;
    rdfs:range rdf:langString ;
    vann:usageNote "USE IN PILOT"@en-US .
    
schema:subOrganization a rdfs:Property ;
    dct:identifier "schema:subOrganization"@en-US ;
    rdfs:label "Sub-Organization"@en-US ;    
    rdfs:comment "A relationship between two organizations where the first includes the second, e.g., as a subsidiary."@en-US ;
    rdfs:isDefinedBy <https://schema.org> ;
    rdfs:domain schema:Organization  ;
    rdfs:range schema:Organization .

jdx:task a rdfs:Property ;
    dct:identifier "jdx:task"@en-US ;
    rdfs:label "Task"@en-US ;    
    rdfs:comment "A piece or unit of work to be done or undertaken and accomplished within a defined period of time or by a deadline; select from an existing enumeration of such types."@en-US ;
    rdfs:isDefinedBy <http://purl.org/jdx/terms/> ;
    rdfs:domain jdx:JobMaster, jdx:JobDescription, jdx:JobCompetenctProfile, jdx:JobPosting ;
    rdfs:range skos:Concept ;
    rdfs:subPropertyOf jdx:competency ;
    vann:usageNote "Use a value selected from a controlled vocabulary of task types such as O*NET tasks; encode using the jdx:AnnotatedDefinedTerm entity."@en-US ;
    vann:usageNote "USE IN PILOT"@en-US .
    
jdx:technology a rdfs:Property ;
    dct:identifier "jdx:technology"@en-US ;
    rdfs:label "Technology"@en-US ;    
    rdfs:comment "Tool, application or other form of technology that requires knowledge, skill and ability to use effectively in executing the tasks and responsibilities of the job; select from an existing enumeration of such types."@en-US ;
    rdfs:isDefinedBy <http://purl.org/jdx/terms/> ;
    rdfs:domain jdx:JobMaster, jdx:JobDescription, jdx:JobPosting ;
    rdfs:range skos:Concept  ;
    vann:usageNote "Use a value selected from a controlled vocabulary of technology types such as O*NET technology and tools; encode using the jdx:AnnotatedDefinedTerm entity."@en-US ;
    vann:usageNote "USE IN PILOT"@en-US .
    
schema:telephone a rdfs:Property ;
    dct:identifier "schema:telephone"@en-US ;
    rdfs:label "Telephone"@en-US ;    
    rdfs:comment "The telephone number of an organization or person."@en-US ;
    rdfs:isDefinedBy <https://schema.org> ;
    rdfs:domain schema:Place, schema:ContactPoint, schema:Organization ;
    rdfs:range xsd:string ;
    vann:usageNote "USE IN PILOT"@en-US .
    
schema:termCode a rdfs:Property ;
    dct:identifier "schema:termCode"@en-US ;
    rdfs:label "Term Code"@en-US ;    
    rdfs:comment "A code that identifies this DefinedTerm within a DefinedTermSet."@en-US ;
    rdfs:isDefinedBy <https://schema.org> ;
    rdfs:domain jdx:AnnotatedDefinedTerm  ;
    rdfs:range xsd:string .
    
schema:title a rdfs:Property ;
    dct:identifier "schema:title"@en-US ;
    rdfs:label "Title"@en-US ;    
    rdfs:comment "The title of the job."@en-US ;
    rdfs:isDefinedBy <https://schema.org> ;
    rdfs:domain jdx:JobMaster, jdx:JobCompetencyProfile, jdx:JobDescription, jdx:JobPosting ;
    rdfs:range rdf:langString ;
    vann:usageNote "USE IN PILOT"@en-US .
    
jdx:travelRequirement a rdfs:Property ;
    dct:identifier "jdx:travelRequirement"@en-US ;
    rdfs:label "Work Travel Requirements"@en-US ;    
    rdfs:comment "Information about any required travel, systematic or occasional."@en-US ;
    rdfs:isDefinedBy <http://purl.org/jdx/terms/> ;
    rdfs:domain jdx:JobMaster, jdx:JobDescription, jdx:JobPosting ;
    rdfs:range rdf:langString .
    
schema:unitText a rdfs:Property ;
    dct:identifier "schema:unitText"@en-US ;
    rdfs:label "Unit Text"@en-US ;    
    rdfs:comment "Unit of measurement on which employee pay is based such as \"hour\", \"day\", \"week\", \"month\", \"year\"; select from an existing enumeration of such types."@en-US ;
    rdfs:isDefinedBy <http://purl.org/jdx/terms/> ;
    rdfs:domain schema:QuantitativeValue ;
    rdfs:range skos:Concept  ;
    vann:usageNote "Google Jobs recommends using \"HOUR\", \"DAY\", \"WEEK\", \"MONTH\", \"YEAR\"; these values also appear in HR Open's PayCycleIntervalCodeList.json"@en-US ;
    vann:usageNote "USE IN PILOT"@en-US .
    
schema:validFrom a rdfs:Property ;
    dct:identifier "schema:validThrough"@en-US ;
    rdfs:label "Valid Through"@en-US ;    
    rdfs:comment "The date from which the item is not valid."@en-US ;
    dct:description: "The date from which the job posting is valid in ISO 8601 format. For example, \"2017-02-24\" or \"2017-02-24T19:33:17+00:00\" (Google) ."@en-US ;
    rdfs:isDefinedBy <https://schema.org> ;
    rdfs:domain jdx:JobPosting ;
    rdfs:range xsd:dateTime ;
    vann:usageNote "USE IN PILOT"@en-US .
    
schema:validThrough a rdfs:Property ;
    dct:identifier "schema:validThrough"@en-US ;
    rdfs:label "Valid Through"@en-US ;    
    rdfs:comment "The date after when [which?] the item is not valid. For example the end of an offer, salary period, or a period of opening hours."@en-US ;
    dct:description: "The date when the job posting will expire in ISO 8601 format. For example, \"2017-02-24\" or \"2017-02-24T19:33:17+00:00\" (Google) ."@en-US ;
    rdfs:isDefinedBy <https://schema.org> ;
    rdfs:domain jdx:JobPosting ;
    rdfs:range xsd:dateTime ;
    vann:usageNote "USE IN PILOT"@en-US .
    
schema:value a rdfs:Property ;
    dct:identifier "schema:value"@en-US ;
    rdfs:label "Value"@en-US ;    
    rdfs:comment "The value of the quantitative value or property value node. (node?)"@en-US ;
    rdfs:isDefinedBy <https://schema.org> ;
    rdfs:domain schema:QuantitativeValue, schema:MonetaryAmount  ;
    rdfs:range xsd:float ;
    vann:usageNote "USE IN PILOT"@en-US .
    
jdx:workActivity a rdfs:Property ;
    dct:identifier "jdx:workActivity"@en-US ;
    rdfs:comment "Work activity asssociated with the job."@en-US ;
    rdfs:isDefinedBy <http://purl.org/jdx/terms/> ;
    rdfs:label "Work Activity"@en-US ;
    rdfs:subPropertyOf jdx:competency ;
    rdfs:domain jdx:JobMaster, jdx:JobDescription, jdx:JobPosting ;
    rdfs:range skos:ConceptScheme  ;
    vann:usageNote "Use a value selected from a controlled vocabulary of activity types such as the O*NET work activities (https://www.onetonline.org/find/descriptor/browse/Work_Activities/); encode using the jdx:AnnotatedDefinedTerm entity."@en-US.
    
jdx:workLanguage a rdfs:Property ;
    dct:identifier "jdx:workLanguage"@en-US ;
    rdfs:label "Work Language"@en-US ;    
    rdfs:comment "Information on the work languages used for the job. (HR)"@en-US ;
    rdfs:isDefinedBy <http://purl.org/jdx/terms/> ;
    rdfs:domain jdx:JobMaster, jdx:JobDescription, jdx:JobPosting ;
    rdfs:range xsd:language ;
    vann:usageNote "USE IN PILOT"@en-US .
    
schema:workHours a rdfs:Property ;
    dct:identifier "schema:workHours"@en-US ;
    rdfs:label "Work Hours"@en-US ;    
    rdfs:comment "The typical working hours for this job (e.g. 1st shift, night shift, 8am-5pm)."@en-US ;
    rdfs:isDefinedBy <https://schema.org> ;
    rdfs:domain jdx:JobMaster, jdx:JobDescription, jdx:JobPosting ;
    rdfs:range rdf:langString ;
    vann:usageNote "USE IN PILOT"@en-US .